logrel definition: using non atomic invariants to model temporary full ownership, and STS to model private/public future world. Updated FTLR accordingly. Added wp rules. Local state encapsulation example (one admit missing).

theories/sts.v
@@ -11,15 +11,17 @@ Definition sts_stateUR := authUR (gmapUR positive (exclR (leibnizC positive))).
 Definition sts_relUR :=
   authUR (gmapUR positive (agreeR (leibnizC (positive → positive → Prop)))).
 
-Definition STS_states := gmap positive positive.
-Definition STS_rels := gmap positive (positive → positive → Prop).
+Definition STS_states : Type := gmap positive positive.
+Definition STS_rels : Type := gmap positive (positive → positive → Prop).
 
 (** The CMRA for the thread pool. *)
 Class STSG Σ :=
   { sts_state_inG :> inG Σ sts_stateUR;
-    sts_rel_inG :> inG Σ sts_relUR;
+    sts_rel_pub_inG :> inG Σ sts_relUR;
+    sts_rel_priv_inG :> inG Σ sts_relUR;
     sts_state_name : gname;
-    sts_rel_name : gname; }.
+    sts_rel_pub_name : gname;
+    sts_rel_priv_name : gname; }.
 
 Section definitionsS.
   Context `{STSG Σ} `{Countable A}.
@@ -30,16 +32,26 @@ Section definitionsS.
   Definition convert_rel (R : A → A → Prop) : positive → positive → Prop :=
     λ x y, ∃ a b, x = encode a ∧ y = encode b ∧ R a b.
 
-  Definition sts_rel (i : positive) (R : A → A → Prop) : iProp Σ :=
-    own (A := sts_relUR) sts_rel_name (◯ {[ i := to_agree (convert_rel R) ]}).
+  Definition sts_rel_pub (i : positive) (R : A → A → Prop) : iProp Σ :=
+    own (A := sts_relUR) sts_rel_pub_name (◯ {[ i := to_agree (convert_rel R) ]}).
+
+  Definition sts_rel_priv (i : positive) (R : A → A → Prop) : iProp Σ :=
+    own (A := sts_relUR) sts_rel_priv_name (◯ {[ i := to_agree (convert_rel R) ]}).
+
+  Definition sts_subset (fr_pub fr_priv : STS_rels) : Prop :=
+    ∀ i (r_pub r_priv : positive → positive → Prop), fr_pub !! i = Some r_pub → fr_priv !! i = Some r_priv →
+                      (∀ a b, r_pub a b → r_priv a b). 
 
   (* very weird bug!!!
      Any two of these conjuncts are ok on their own but not all three!
      But, it works with program!!!!!!!!!!! *)
-  Program Definition sts_full `{STSG Σ} (fs : STS_states) (fr : STS_rels) : iProp Σ
-    := (⌜dom (gset positive) fs = dom (gset positive) fr⌝
+  Program Definition sts_full `{STSG Σ} (fs : STS_states) (fr_pub fr_priv : STS_rels) : iProp Σ
+    := ((⌜dom (gset positive) fs = dom (gset positive) fr_priv⌝ ∧ 
+        ⌜dom (gset positive) fr_priv = dom (gset positive) fr_pub⌝)
+        ∗ ⌜sts_subset fr_pub fr_priv⌝
         ∗ own (A := sts_stateUR) sts_state_name (● (Excl <$> fs))
-          ∗ own (A := sts_relUR) sts_rel_name (● (to_agree <$> fr)))%I.
+        ∗ own (A := sts_relUR) sts_rel_pub_name (● (to_agree <$> fr_pub))
+        ∗ own (A := sts_relUR) sts_rel_priv_name (● (to_agree <$> fr_priv)))%I.
 
   Definition related_sts (fs gs : STS_states) (fr gr : STS_rels) : Prop :=
     dom (gset positive) fs ⊆ dom (gset positive) gs ∧
@@ -47,31 +59,60 @@ Section definitionsS.
     ∀ i x y r r', fs !! i = Some x → gs !! i = Some y →
                   fr !! i = Some r → gr !! i = Some r' → r = r' ∧ rtc r x y.
 
-  Global Instance sts_rel_Persistent i R : Persistent (sts_rel i R).
+  Global Instance sts_rel_pub_Persistent i R : Persistent (sts_rel_pub i R).
   Proof. apply _. Qed.
 
-  Global Instance sts_rel_Timeless i R : Timeless (sts_rel i R).
+  Global Instance sts_rel_priv_Persistent i R : Persistent (sts_rel_priv i R).
+  Proof. apply _. Qed.
+
+  Global Instance sts_rel_pub_Timeless i R : Timeless (sts_rel_pub i R).
+  Proof. apply _. Qed.
+
+  Global Instance sts_rel_priv_Timeless i R : Timeless (sts_rel_priv i R).
   Proof. apply _. Qed.
 
   Global Instance sts_state_Timeless i x : Timeless (sts_state i x).
   Proof. apply _. Qed.
 
-  Global Instance sts_full_Timeless fs fr : Timeless (sts_full fs fr).
+  Global Instance sts_full_Timeless fs fr_pub fr_priv : Timeless (sts_full fs fr_pub fr_priv).
   Proof. apply _. Qed.
 
 End definitionsS.
 
-Typeclasses Opaque sts_state sts_rel sts_full related_sts.
+Typeclasses Opaque sts_state sts_rel_pub sts_rel_priv sts_full related_sts.
+
+Lemma rtc_implies {A : Type} (R Q : A → A → Prop) (x y : A) :
+  (∀ r q, R r q → Q r q) →
+  rtc R x y → rtc Q x y.
+Proof.
+  intros Himpl HR.
+  induction HR.
+  - done.
+  - apply Himpl in H.
+    apply rtc_once in H. 
+    apply rtc_transitive with y; auto.
+Qed. 
 
 Section STS.
   Context `{STSG Σ} `{Countable A}.
   Implicit Types x y : positive.
   Implicit Types a b : A.
   Implicit Types fs gs : STS_states.
-  Implicit Types fr gr : STS_rels.
-  Implicit Types R : A → A → Prop.
+  Implicit Types fr_pub fr_priv gr_pub gr_priv : STS_rels.
+  Implicit Types R Q : A → A → Prop.
   Implicit Types Rp : positive → positive → Prop.
 
+  Lemma elem_of_gmap_dom {K V : Type} `{EqDecision K} `{Countable K}
+        (m : gmap K V) (i : K) :
+    is_Some (m !! i) ↔ i ∈ dom (gset K) m.  
+  Proof.
+    split.
+    - intros [x Hsome].
+      apply elem_of_dom. eauto.
+    - intros Hin.
+      by apply elem_of_dom in Hin. 
+  Qed. 
+      
   Lemma related_sts_refl fs fr : related_sts fs fs fr fr.
   Proof.
     split; [|split]; trivial.
@@ -90,18 +131,18 @@ Section STS.
     split; etrans; eauto.
   Qed.
 
-  Lemma sts_full_rel fs fr i R :
-    sts_full fs fr -∗ sts_rel i R -∗ ⌜fr !! i = Some (convert_rel R)⌝.
+  Lemma sts_full_rel_priv fs fr_pub fr_priv i R :
+    sts_full fs fr_pub fr_priv -∗ sts_rel_priv i R -∗ ⌜fr_priv !! i = Some (convert_rel R)⌝.
   Proof.
-    rewrite /sts_full /sts_rel.
-    iIntros "[% [_ H1]] H2".
+    rewrite /sts_full /sts_rel_priv.
+    iIntros "[% [_ (_ & _ & H1)]] H2".
     iDestruct (own_valid_2 with "H1 H2") as %[HR Hv]%auth_valid_discrete;
       iPureIntro.
     specialize (Hv i).
     revert HR; rewrite /= left_id singleton_included;
       intros [z [Hz HR]]; revert HR; rewrite Some_included_total; intros HR.
     rewrite lookup_fmap in Hz, Hv.
-    destruct (fr !! i) eqn:Heq; rewrite Heq /= in Hz, Hv; last by inversion Hz.
+    destruct (fr_priv !! i) eqn:Heq; rewrite Heq /= in Hz, Hv; last by inversion Hz.
     revert Hv; rewrite Hz; intros [u Hu]%to_agree_uninj.
     revert HR; rewrite -Hu; intros HR%to_agree_included%leibniz_equiv;
       simplify_eq.
@@ -110,11 +151,65 @@ Section STS.
     by eauto.
   Qed.
 
-  Lemma sts_full_state fs fr i a :
-    sts_full fs fr -∗ sts_state i a -∗ ⌜fs !! i = Some (encode a)⌝.
+   Lemma sts_full_rel_pub fs fr_pub fr_priv i R :
+    sts_full fs fr_pub fr_priv -∗ sts_rel_pub i R -∗ ⌜fr_pub !! i = Some (convert_rel R)⌝.
+  Proof.
+    rewrite /sts_full /sts_rel_pub.
+    iIntros "[% [_ (_ & H1 & _)]] H2".
+    iDestruct (own_valid_2 with "H1 H2") as %[HR Hv]%auth_valid_discrete;
+      iPureIntro.
+    specialize (Hv i).
+    revert HR; rewrite /= left_id singleton_included;
+      intros [z [Hz HR]]; revert HR; rewrite Some_included_total; intros HR.
+    rewrite lookup_fmap in Hz, Hv.
+    destruct (fr_pub !! i) eqn:Heq; rewrite Heq /= in Hz, Hv; last by inversion Hz.
+    revert Hv; rewrite Hz; intros [u Hu]%to_agree_uninj.
+    revert HR; rewrite -Hu; intros HR%to_agree_included%leibniz_equiv;
+      simplify_eq.
+    inversion Hz as [? ? Hz'|]; simplify_eq.
+    revert Hz'; rewrite -Hu; intros Hz'%to_agree_inj%leibniz_equiv; simplify_eq.
+    by eauto.
+  Qed.
+
+  Lemma sts_full_rel_pub_priv fs fr_pub fr_priv gs gr_pub gr_priv :
+    sts_full fs fr_pub fr_priv -∗
+    ⌜related_sts fs gs fr_pub gr_pub⌝ -∗
+    sts_full gs gr_pub gr_priv -∗
+    ⌜∀ i fi gi, fr_priv !! i = Some fi → gr_priv !! i = Some gi → fi = gi⌝ -∗
+    ⌜related_sts fs gs fr_priv gr_priv⌝.
+  Proof.
+    iIntros "Hffull % Hgfull %". destruct a as (Hfs & Hfrpub & Hrel). 
+    rename a0 into Hpriv. 
+    rewrite /sts_full.
+    iDestruct "Hgfull" as "([% %] & % & _ & _)".
+    iDestruct "Hffull" as "([% %] & % & _ & _)".
+    iPureIntro. 
+    split; auto. split.
+    - by rewrite H2 H5. 
+    - intros i x y r_priv r_priv' Hfsi Hgsi Hfr_privi Hgr_privi.
+      rewrite /sts_subset in H6, H3.
+      assert (is_Some (gr_pub !! i)) as [gr_pub_i Hsomeg].
+      { assert (i ∈ dom (gset positive) gr_priv); [apply elem_of_gmap_dom;eauto|]. 
+        apply elem_of_gmap_dom. by rewrite -H2. }
+      assert (is_Some (fr_pub !! i)) as [fr_pub_i Hsomef].
+      { assert (i ∈ dom (gset positive) fr_priv); [apply elem_of_gmap_dom;eauto|]. 
+        apply elem_of_gmap_dom. by rewrite -H5. }
+      (* specialize H3 with i gr_pub_i r_priv' x y. *)
+      (* specialize H6 with i gr_pub_i r_priv x y. *)
+      assert (fr_pub_i = gr_pub_i ∧ rtc fr_pub_i x y) as [Hfrgrpub Hxy];
+        [apply Hrel with i; auto|].
+      assert (r_priv = r_priv');
+        [apply Hpriv with i; auto|].
+      split; auto.
+      apply rtc_implies with gr_pub_i; try congruence.
+        apply H3 with i; try congruence.  
+  Qed. 
+      
+  Lemma sts_full_state fs fr_pub fr_priv i a :
+    sts_full fs fr_pub fr_priv -∗ sts_state i a -∗ ⌜fs !! i = Some (encode a)⌝.
   Proof.
     rewrite /sts_full /sts_state.
-    iIntros "[% [H1 _]] H2".
+    iIntros "[% [_ [H1 _]]] H2".
     iDestruct (own_valid_2 with "H1 H2") as %[HR Hv]%auth_valid_discrete;
       iPureIntro.
     specialize (Hv i).
@@ -127,15 +222,19 @@ Section STS.
     apply leibniz_equiv in HR; simplify_eq; eauto.
   Qed.
 
-  Lemma sts_alloc fs fr a R :
-    sts_full fs fr ==∗
-             ∃ i, sts_full (<[i := encode a ]>fs) (<[i := convert_rel R ]>fr)
-                  ∗ ⌜i ∉ dom (gset positive) fs⌝ ∗ ⌜i ∉ dom (gset positive) fr⌝
-                  ∗ sts_state i a ∗ sts_rel i R.
+  Lemma sts_alloc fs fr_pub fr_priv a R Q :
+    (∀ x y, (convert_rel R) x y → (convert_rel Q) x y) →
+    sts_full fs fr_pub fr_priv ==∗
+             ∃ i, sts_full (<[i := encode a ]>fs) (<[i := convert_rel R ]>fr_pub)
+                           (<[i := convert_rel Q ]>fr_priv)
+                           ∗ ⌜i ∉ dom (gset positive) fs⌝
+                           ∗ ⌜i ∉ dom (gset positive) fr_pub⌝
+                           ∗ ⌜i ∉ dom (gset positive) fr_priv⌝
+                  ∗ sts_state i a ∗ sts_rel_pub i R ∗ sts_rel_priv i Q.
   Proof.
-    rewrite /sts_full /sts_rel /sts_state.
-    iIntros "[Hd [H1 H2]]".
-    iDestruct "Hd" as %Hd.
+    rewrite /sts_full /sts_rel_pub /sts_rel_priv /sts_state.
+    iIntros (HRQ) "[Hd [% [H1 [H2 H2']]]]".
+    iDestruct "Hd" as %[Hd Hd'].
     iMod (own_update
             (A := sts_stateUR)
             _ _
@@ -153,36 +252,58 @@ Section STS.
             (A := sts_relUR)
             _ _
             (● (to_agree <$>
-                <[fresh (dom (gset positive) fs) := convert_rel R]> fr)
+                <[fresh (dom (gset positive) fs) := convert_rel R]> fr_pub)
             ⋅ ◯ {[fresh (dom (gset positive) fs) := to_agree (convert_rel R)]})
             with "H2") as "[H2 Hr]".
     { apply auth_update_alloc.
       rewrite fmap_insert /=.
       apply: alloc_singleton_local_update; last done.
       apply (not_elem_of_dom (D := gset positive)).
-      rewrite dom_fmap Hd.
+      rewrite dom_fmap Hd Hd'.
+      apply is_fresh. }
+    iMod (own_update
+            (A := sts_relUR)
+            _ _
+            (● (to_agree <$>
+                <[fresh (dom (gset positive) fs) := convert_rel Q]> fr_priv)
+            ⋅ ◯ {[fresh (dom (gset positive) fs) := to_agree (convert_rel Q)]})
+            with "H2'") as "[H2' Hr']".
+    { apply auth_update_alloc.
+      rewrite fmap_insert /=.
+      apply: alloc_singleton_local_update; last done.
+      apply (not_elem_of_dom (D := gset positive)).
+      rewrite dom_fmap Hd Hd'.
       apply is_fresh. }
     iModIntro.
     iExists _; iFrame.
-    repeat iSplit; iPureIntro;
-      rewrite ?dom_insert_L ?Hd; by try apply is_fresh.
+    repeat iSplit; try iPureIntro;
+      rewrite ?dom_insert_L ?Hd Hd'; try apply is_fresh; auto.
+    rewrite /sts_subset.
+    intros i r_pub r_priv Hpub Hpriv a' b' Ha'.
+    destruct (decide (fresh (dom (gset positive) fr_pub) = i)).
+    - rewrite e lookup_insert in Hpub, Hpriv. rewrite lookup_insert in Hpriv.
+      inversion Hpub; inversion Hpriv.
+      apply HRQ. congruence.
+    - rewrite lookup_insert_ne in Hpub; auto.
+      rewrite lookup_insert_ne in Hpriv; auto.
+      rewrite /sts_subset in H1. apply H1 with i r_pub; auto. 
   Qed.
 
-  Lemma sts_update fs fr i a b :
-    sts_full fs fr -∗ sts_state i a ==∗
-    sts_full (<[i := encode b ]>fs) fr ∗ sts_state i b.
+  Lemma sts_update fs fr_pub fr_priv i a b :
+    sts_full fs fr_pub fr_priv -∗ sts_state i a ==∗
+    sts_full (<[i := encode b ]>fs) fr_pub fr_priv ∗ sts_state i b.
   Proof.
     iIntros "Hsf Hi".
     iDestruct (sts_full_state with "Hsf Hi") as %Hfs.
-    rewrite /sts_full /sts_rel /sts_state.
-    iDestruct "Hsf" as "[Hd [H1 H2]]".
+    rewrite /sts_full /sts_rel_pub /sts_rel_priv /sts_state.
+    iDestruct "Hsf" as "[Hd [H1 [H2 [H3 H4]]]]".
     iDestruct "Hd" as %Hd.
-    iCombine "H1" "Hi" as "H1".
+    iCombine "H2" "Hi" as "H2".
     iMod (own_update (A := sts_stateUR)
             _ _
             (● (<[i := Excl (encode b)]> (Excl <$> fs))
                ⋅ ◯ {[i := Excl (encode b)]})
-            with "H1") as "[H1 Hs]".
+            with "H2") as "[H2 Hs]".
     { apply auth_update.
       apply: singleton_local_update; eauto.
       rewrite lookup_fmap Hfs //=.
