theories/addr_reg_sample.v
@@ -1,0 +1,486 @@
+From stdpp Require Import gmap fin_maps list.
+From cap_machine Require Export addr_reg lang.
+From iris.proofmode Require Import tactics.
+Require Import Eqdep_dec List.
+
+  (* Some addresses *)
+  Definition a0 : Addr := A 0 eq_refl.
+  Definition a1 : Addr := A 1 eq_refl.
+  Definition a2 : Addr := A 2 eq_refl.
+  Definition a3 : Addr := A 3 eq_refl.
+  Definition a4 : Addr := A 4 eq_refl.
+  Definition a5 : Addr := A 5 eq_refl.
+  Definition a6 : Addr := A 6 eq_refl.
+  Definition a7 : Addr := A 7 eq_refl.
+  Definition a8 : Addr := A 8 eq_refl.
+  Definition a9 : Addr := A 9 eq_refl.
+  Definition a10 : Addr := A 10 eq_refl.
+  Definition a11 : Addr := A 11 eq_refl.
+  Definition a12 : Addr := A 12 eq_refl.
+  Definition a13 : Addr := A 13 eq_refl.
+  Definition a14 : Addr := A 14 eq_refl.
+  Definition a15 : Addr := A 15 eq_refl.
+  Definition a16 : Addr := A 16 eq_refl.
+  Definition a17 : Addr := A 17 eq_refl.
+  Definition a18 : Addr := A 18 eq_refl.
+  Definition a19 : Addr := A 19 eq_refl.
+  Definition a20 : Addr := A 20 eq_refl.
+  Definition a21 : Addr := A 21 eq_refl.
+  Definition a22 : Addr := A 22 eq_refl.
+  Definition a23 : Addr := A 23 eq_refl.
+  Definition a24 : Addr := A 24 eq_refl.
+  Definition a25 : Addr := A 25 eq_refl.
+  Definition a26 : Addr := A 26 eq_refl.
+  Definition a27 : Addr := A 27 eq_refl.
+  Definition a28 : Addr := A 28 eq_refl.
+  Definition a29 : Addr := A 29 eq_refl.
+  Definition a30 : Addr := A 30 eq_refl.
+  Definition a31 : Addr := A 31 eq_refl.
+  Definition a32 : Addr := A 32 eq_refl.
+  Definition a33 : Addr := A 33 eq_refl.
+  Definition a34 : Addr := A 34 eq_refl.
+  Definition a35 : Addr := A 35 eq_refl.
+  Definition a36 : Addr := A 36 eq_refl.
+  Definition a37 : Addr := A 37 eq_refl.
+  Definition a38 : Addr := A 38 eq_refl.
+  Definition a39 : Addr := A 39 eq_refl.
+  Definition a40 : Addr := A 40 eq_refl.
+  Definition a41 : Addr := A 41 eq_refl.
+  Definition a42 : Addr := A 42 eq_refl.
+  Definition a43 : Addr := A 43 eq_refl.
+  Definition a44 : Addr := A 44 eq_refl.
+  Definition a45 : Addr := A 45 eq_refl.
+  Definition a46 : Addr := A 46 eq_refl.
+  Definition a47 : Addr := A 47 eq_refl.
+  Definition a48 : Addr := A 48 eq_refl.
+  Definition a49 : Addr := A 49 eq_refl.
+  Definition a50 : Addr := A 50 eq_refl.
+  Definition a51 : Addr := A 51 eq_refl.
+  Definition a52 : Addr := A 52 eq_refl.
+  Definition a53 : Addr := A 53 eq_refl.
+  Definition a54 : Addr := A 54 eq_refl.
+  Definition a55 : Addr := A 55 eq_refl.
+  Definition a56 : Addr := A 56 eq_refl.
+  Definition a57 : Addr := A 57 eq_refl.
+  Definition a58 : Addr := A 58 eq_refl.
+  Definition a59 : Addr := A 59 eq_refl.
+  Definition a60 : Addr := A 60 eq_refl.
+  Definition a61 : Addr := A 61 eq_refl.
+  Definition a62 : Addr := A 62 eq_refl.
+  Definition a63 : Addr := A 63 eq_refl.
+  Definition a64 : Addr := A 64 eq_refl.
+  Definition a65 : Addr := A 65 eq_refl.
+  Definition a66 : Addr := A 66 eq_refl.
+  Definition a67 : Addr := A 67 eq_refl.
+  Definition a68 : Addr := A 68 eq_refl.
+  Definition a69 : Addr := A 69 eq_refl.
+  Definition a70 : Addr := A 70 eq_refl.
+  Definition a71 : Addr := A 71 eq_refl.
+  Definition a72 : Addr := A 72 eq_refl.
+  Definition a73 : Addr := A 73 eq_refl.
+  Definition a74 : Addr := A 74 eq_refl.
+  Definition a75 : Addr := A 75 eq_refl.
+  Definition a76 : Addr := A 76 eq_refl.
+  Definition a77 : Addr := A 77 eq_refl.
+  Definition a78 : Addr := A 78 eq_refl.
+  Definition a79 : Addr := A 79 eq_refl.
+  Definition a80 : Addr := A 80 eq_refl.
+  Definition a81 : Addr := A 81 eq_refl.
+  Definition a82 : Addr := A 82 eq_refl.
+  Definition a83 : Addr := A 83 eq_refl.
+  Definition a84 : Addr := A 84 eq_refl.
+  Definition a85 : Addr := A 85 eq_refl.
+  Definition a86 : Addr := A 86 eq_refl.
+  Definition a87 : Addr := A 87 eq_refl.
+  Definition a88 : Addr := A 88 eq_refl.
+  Definition a89 : Addr := A 89 eq_refl.
+  Definition a90 : Addr := A 90 eq_refl.
+  Definition a91 : Addr := A 91 eq_refl.
+  Definition a92 : Addr := A 92 eq_refl.
+  Definition a93 : Addr := A 93 eq_refl.
+  Definition a94 : Addr := A 94 eq_refl.
+  Definition a95 : Addr := A 95 eq_refl.
+  Definition a96 : Addr := A 96 eq_refl.
+  Definition a97 : Addr := A 97 eq_refl.
+  Definition a98 : Addr := A 98 eq_refl.
+  Definition a99 : Addr := A 99 eq_refl.
+  Definition a100 : Addr := A 100 eq_refl.
+  Definition a101 : Addr := A 101 eq_refl.
+  Definition a102 : Addr := A 102 eq_refl.
+  Definition a103 : Addr := A 103 eq_refl.
+  Definition a104 : Addr := A 104 eq_refl.
+  Definition a105 : Addr := A 105 eq_refl.
+  Definition a106 : Addr := A 106 eq_refl.
+  Definition a107 : Addr := A 107 eq_refl.
+  Definition a108 : Addr := A 108 eq_refl.
+  Definition a109 : Addr := A 109 eq_refl.
+  Definition a110 : Addr := A 110 eq_refl.
+  Definition a111 : Addr := A 111 eq_refl.
+  Definition a112 : Addr := A 112 eq_refl.
+  Definition a113 : Addr := A 113 eq_refl.
+  Definition a114 : Addr := A 114 eq_refl.
+  Definition a115 : Addr := A 115 eq_refl.
+  Definition a116 : Addr := A 116 eq_refl.
+  Definition a117 : Addr := A 117 eq_refl.
+  Definition a118 : Addr := A 118 eq_refl.
+  Definition a119 : Addr := A 119 eq_refl.
+  Definition a120 : Addr := A 120 eq_refl.
+  Definition a121 : Addr := A 121 eq_refl.
+  Definition a122 : Addr := A 122 eq_refl.
+  Definition a123 : Addr := A 123 eq_refl.
+  Definition a124 : Addr := A 124 eq_refl.
+  Definition a125 : Addr := A 125 eq_refl.
+  Definition a126 : Addr := A 126 eq_refl.
+  Definition a127 : Addr := A 127 eq_refl.
+  Definition a128 : Addr := A 128 eq_refl.
+  Definition a129 : Addr := A 129 eq_refl.
+  Definition a130 : Addr := A 130 eq_refl.
+  Definition a131 : Addr := A 131 eq_refl.
+  Definition a132 : Addr := A 132 eq_refl.
+  Definition a133 : Addr := A 133 eq_refl.
+  Definition a134 : Addr := A 134 eq_refl.
+  Definition a135 : Addr := A 135 eq_refl.
+  Definition a136 : Addr := A 136 eq_refl.
+  Definition a137 : Addr := A 137 eq_refl.
+  Definition a138 : Addr := A 138 eq_refl.
+  Definition a139 : Addr := A 139 eq_refl.
+  Definition a140 : Addr := A 140 eq_refl.
+  Definition a141 : Addr := A 141 eq_refl.
+  Definition a142 : Addr := A 142 eq_refl.
+  Definition a143 : Addr := A 143 eq_refl.
+  Definition a144 : Addr := A 144 eq_refl.
+  Definition a145 : Addr := A 145 eq_refl.
+  Definition a146 : Addr := A 146 eq_refl.
+  Definition a147 : Addr := A 147 eq_refl.
+  Definition a148 : Addr := A 148 eq_refl.
+  Definition a149 : Addr := A 149 eq_refl.
+  Definition a150 : Addr := A 150 eq_refl.
+  Definition a151 : Addr := A 151 eq_refl.
+  Definition a152 : Addr := A 152 eq_refl.
+  Definition a153 : Addr := A 153 eq_refl.
+  Definition a154 : Addr := A 154 eq_refl.
+  Definition a155 : Addr := A 155 eq_refl.
+  Definition a156 : Addr := A 156 eq_refl.
+  Definition a157 : Addr := A 157 eq_refl.
+  Definition a158 : Addr := A 158 eq_refl.
+  Definition a159 : Addr := A 159 eq_refl.
+  Definition a160 : Addr := A 160 eq_refl.
+
+  Lemma a0a1 : (a0 + 1)%a = Some a1.
+  Proof.
+    unfold incr_addr. simpl. do 2 f_equal. apply eq_proofs_unicity. decide equality.
+  Qed.
+  
+  (* Some general purpuse registers *)
+  Definition r_t0 : RegName := R 0 eq_refl. 
+  Definition r_t1 : RegName := R 1 eq_refl.
+  Definition r_t2 : RegName := R 2 eq_refl.
+  Definition r_t3 : RegName := R 3 eq_refl.
+  Definition r_t4 : RegName := R 4 eq_refl.
+  Definition r_t5 : RegName := R 5 eq_refl.
+  Definition r_t6 : RegName := R 6 eq_refl.
+  Definition r_t7 : RegName := R 7 eq_refl.
+  Definition r_t8 : RegName := R 8 eq_refl.
+  Definition r_t9 : RegName := R 9 eq_refl.
+  Definition r_t10 : RegName := R 10 eq_refl.
+  Definition r_t11 : RegName := R 11 eq_refl.
+  Definition r_t12 : RegName := R 12 eq_refl.
+  Definition r_t13 : RegName := R 13 eq_refl.
+  Definition r_t14 : RegName := R 14 eq_refl.
+  Definition r_t15 : RegName := R 15 eq_refl.
+  Definition r_t16 : RegName := R 16 eq_refl.
+  Definition r_t17 : RegName := R 17 eq_refl.
+  Definition r_t18 : RegName := R 18 eq_refl.
+  Definition r_t19 : RegName := R 19 eq_refl.
+  Definition r_t20 : RegName := R 20 eq_refl.
+  Definition r_t21 : RegName := R 21 eq_refl.
+  Definition r_t22 : RegName := R 22 eq_refl.
+  Definition r_t23 : RegName := R 23 eq_refl.
+  Definition r_t24 : RegName := R 24 eq_refl.
+  Definition r_t25 : RegName := R 25 eq_refl.
+  Definition r_t26 : RegName := R 26 eq_refl.
+  Definition r_t27 : RegName := R 27 eq_refl.
+  Definition r_t28 : RegName := R 28 eq_refl.
+  Definition r_t29 : RegName := R 29 eq_refl.
+  Definition r_t30 : RegName := R 30 eq_refl.
+  Definition r_t31 : RegName := R 31 eq_refl.
+
+  (* A list of all general purpuse registers (if regnum=31) *)
+  Definition all_registers : list RegName :=
+    [r_t0;r_t1;r_t2;r_t3;r_t4;r_t5;r_t6;r_t7;r_t8;r_t9;r_t10;r_t11;r_t12;r_t13;
+       r_t14;r_t15;r_t16;r_t17;r_t18;r_t19;r_t20;r_t21;r_t22;r_t23;r_t24;r_t25;r_t26;
+         r_t27;r_t28;r_t29;r_t30;r_t31;PC].
+
+
+  (* Instructions and their decodings *)
+  (* A special register for the stack pointer, different from PC *)
+  Definition r_stk : RegName := r_t31.
+  Lemma r_stk_ne : r_stk ≠ PC. Proof. done. Qed. 
+
+  (* Restore code encodings *)
+  Parameter w_1 : Z.
+  Parameter w_2 : Z.
+  Parameter w_3 : Z.
+  Parameter w_4a : Z.
+  Parameter w_4b : Z.
+  Parameter w_4c : Z.
+  Parameter local_e : Z. 
+  (* Instruction encodings *)
+  Parameter lea_z : RegName → Z → Word.
+  Parameter lea_r : RegName → RegName → Word.
+  Parameter store_z : RegName → Z → Word.
+  Parameter store_r : RegName → RegName → Word.
+  Parameter load_r : RegName → RegName → Word.
+  Parameter move_z : RegName → Z → Word.
+  Parameter move_r : RegName → RegName → Word.
+  Parameter restrict_r : RegName → RegName → Word.
+  Parameter restrict_z : RegName → Z → Word.
+  Parameter geta : RegName → RegName → Word.
+  Parameter getb : RegName → RegName → Word.
+  Parameter gete : RegName → RegName → Word. 
+  Parameter add_r_z : RegName → RegName → Z → Word.
+  Parameter sub_r_r : RegName → RegName → RegName → Word.
+  Parameter sub_r_z : RegName → RegName → Z → Word.
+  Parameter sub_z_z : RegName → Z → Z → Word.
+  Parameter subseg_r_r : RegName → RegName → RegName → Word.
+  Parameter jnz : RegName → RegName → Word.
+  Parameter lt_r_r : RegName → RegName → RegName → Word.
+  Parameter jmp : RegName → Word.
+  Parameter halt : Word.
+  Parameter fail_end : Word. 
+  (* Encoding decodings *)
+  Axiom halt_i : cap_lang.decode (halt) = Halt.
+  Axiom fail_end_i : cap_lang.decode (fail_end) = Fail.
+  Axiom jnz_i : ∀ r1 r2, cap_lang.decode (jnz r1 r2) = Jnz r1 r2.
+  Axiom lt_i : ∀ dst r1 r2, cap_lang.decode (lt_r_r dst r1 r2) = Lt dst (inr r1) (inr r2).
+  Axiom jmp_i : ∀ r, cap_lang.decode (jmp r) = Jmp r. 
+  Axiom lea_z_i : ∀ r z, cap_lang.decode (lea_z r z) = Lea r (inl z).
+  Axiom lea_r_i : ∀ r1 r2, cap_lang.decode (lea_r r1 r2) = Lea r1 (inr r2). 
+  Axiom store_z_i : ∀ r z, cap_lang.decode (store_z r z) = Store r (inl z).
+  Axiom store_r_i : ∀ r1 r2, cap_lang.decode (store_r r1 r2) = Store r1 (inr r2).
+  Axiom load_r_i : ∀ r1 r2, cap_lang.decode (load_r r1 r2) = Load r1 r2.
+  Axiom move_z_i : ∀ r z, cap_lang.decode (move_z r z) = Mov r (inl z).
+  Axiom move_r_i : ∀ r1 r2, cap_lang.decode (move_r r1 r2) = Mov r1 (inr r2).
+  Axiom restrict_r_i : ∀ r1 r2, cap_lang.decode (restrict_r r1 r2) = Restrict r1 (inr r2).
+  Axiom restrict_r_z : ∀ r1 z, cap_lang.decode (restrict_z r1 z) = Restrict r1 (inl z).
+  Axiom geta_i : ∀ r1 r2, cap_lang.decode (geta r1 r2) = GetA r1 r2.
+  Axiom getb_i : ∀ r1 r2, cap_lang.decode (getb r1 r2) = GetB r1 r2.
+  Axiom gete_i : ∀ r1 r2, cap_lang.decode (gete r1 r2) = GetE r1 r2. 
+  Axiom add_r_z_i : ∀ r1 r2 z, cap_lang.decode (add_r_z r1 r2 z) = cap_lang.Add r1 (inr r2) (inl z).
+  Axiom sub_r_r_i : ∀ r1 r2 r3, cap_lang.decode (sub_r_r r1 r2 r3) = cap_lang.Sub r1 (inr r2) (inr r3).
+  Axiom sub_z_z_i : ∀ r1 z1 z2, cap_lang.decode (sub_z_z r1 z1 z2) = cap_lang.Sub r1 (inl z1) (inl z2).
+  Axiom sub_r_z_i : ∀ r1 r2 z1, cap_lang.decode (sub_r_z r1 r2 z1) = cap_lang.Sub r1 (inr r2) (inl z1).
+  Axiom subseg_r_r_i : ∀ r1 r2 r3, cap_lang.decode (subseg_r_r r1 r2 r3) = Subseg r1 (inr r2) (inr r3). 
+  (* encodings of restore code *)
+  Axiom i_1 : cap_lang.encode (Mov r_t1 (inr PC)) = inl w_1. 
+  Axiom i_2 : cap_lang.encode (Lea r_t1 (inl 7%Z)) = inl w_2.
+  Axiom i_3 : cap_lang.encode (Load r_stk r_t1) = inl w_3.
+  Axiom i_4a : cap_lang.encode (Sub (r_t1) (inl 0%Z) (inl 1%Z)) = inl w_4a.
+  Axiom i_4b : cap_lang.encode (Lea r_stk (inr r_t1)) = inl w_4b.
+  Axiom i_4c : cap_lang.encode (Load PC r_stk) = inl w_4c.
+  
+  (* encodings of return pointer permission pair *)
+  Axiom epp_local_e : cap_lang.decodePermPair local_e = (E,Local).
+
+
+
+
+  
+   Lemma not_elem_of_list {A : Type} `{EqDecision A} (a : A) (l x : list A) :
+     a ∈ x → a ∉ list_difference l x.
+   Proof.
+     intros Hax.
+     rewrite /not.
+     intros Hal.
+     by apply elem_of_list_difference in Hal as [Ha' Hax_not].
+   Qed.
+
+   Lemma list_difference_nil {A : Type} `{EqDecision A} (l : list A) :
+     list_difference l [] = l.
+   Proof.
+     induction l; auto.
+     simpl. f_equal.
+     apply IHl.
+   Qed. 
+
+   Lemma list_difference_length_cons {A : Type} `{EqDecision A}
+         (l2 : list A) (a : A) :
+     list_difference [a] (a :: l2) = []. 
+   Proof.
+     simpl.
+     assert (a ∈ a :: l2); first apply elem_of_list_here. 
+     destruct (decide_rel elem_of a (a :: l2)); auto; last contradiction.  
+   Qed.
+
+   Lemma list_difference_skip {A : Type} `{EqDecision A}
+         (l1 l2 : list A) (b : A) :
+     ¬ (b ∈ l1) →
+     list_difference l1 (b :: l2) = list_difference l1 l2.
+   Proof.
+     intros Hnin.
+     induction l1; auto.
+     apply not_elem_of_cons in Hnin.
+     destruct Hnin as [Hne Hl1].
+     simpl.
+     destruct (decide_rel elem_of a (b :: l2)).
+     - apply elem_of_cons in e.
+       destruct e as [Hcontr | Hl2]; first congruence.
+       destruct (decide_rel elem_of a l2); last contradiction.
+         by apply IHl1.
+     - apply not_elem_of_cons in n.
+       destruct n as [Hne' Hl2].
+       destruct (decide_rel elem_of a l2); first contradiction.
+       f_equal.
+         by apply IHl1.
+   Qed. 
+
+   Lemma list_difference_nested {A : Type} `{EqDecision A}
+         (l1 l1' l2 : list A) (b : A) :
+     ¬ (b ∈ (l1 ++ l1')) →
+     list_difference (l1 ++ b :: l1') (b :: l2) = list_difference (l1 ++ l1') l2.
+   Proof.
+     intros Hnotin.
+     induction l1.
+     - simpl.
+       assert (b ∈ (b :: l2)); first apply elem_of_list_here.
+       destruct (decide_rel elem_of b (b :: l2)); last contradiction.
+       rewrite list_difference_skip; auto.
+     - simpl in *.
+       apply not_elem_of_cons in Hnotin.
+       destruct Hnotin as [Hne Hnotin]. 
+       destruct (decide_rel elem_of a (b :: l2)).
+       + apply elem_of_cons in e.
+         destruct e as [Hcontr | Hl2]; first congruence.
+         destruct (decide_rel elem_of a l2); last contradiction.
+           by apply IHl1.
+       + apply not_elem_of_cons in n.
+         destruct n as [Hne' Hnotin'].
+         destruct (decide_rel elem_of a l2); first contradiction.
+         f_equal. 
+           by apply IHl1.
+   Qed. 
+
+   Lemma list_difference_length_ni  {A : Type} `{EqDecision A}
+         (l1 : list A) (b : A) :
+     ¬ (b ∈ l1) →
+     length (list_difference l1 [b]) = length l1.
+   Proof.
+     intros Hna.
+     destruct l1; auto. 
+     simpl.
+     apply not_elem_of_cons in Hna.
+     destruct Hna as [Hne Hna].
+     destruct (decide_rel elem_of a [b]).
+     - apply elem_of_list_singleton in e. congruence.
+     - simpl. rewrite list_difference_skip; auto.
+         by rewrite list_difference_nil.
+   Qed.        
+   
+   Lemma list_difference_length {A : Type} `{EqDecision A}
+         (l1 : list A) (b : A) :
+     b ∈ l1 →
+     NoDup l1 →
+     length (list_difference l1 [b]) =
+     length l1 - 1.
+   Proof.
+     intros Ha Hndup.
+     induction l1; auto.
+     destruct (decide (b = a)).
+     - subst.
+       assert (a ∈ a :: l1); first apply elem_of_list_here.
+       apply NoDup_cons_iff in Hndup.
+       destruct Hndup as [Hni Hndup].
+       assert (¬ (a ∈ l1)) as Hni'.
+       { rewrite /not. intros Hin. apply elem_of_list_In in Hin. contradiction. }
+       simpl.
+       assert (a ∈ [a]); first apply elem_of_list_here.
+       destruct (decide_rel elem_of a [a]); last contradiction.
+       rewrite -minus_n_O. 
+       apply list_difference_length_ni; auto.
+     - simpl.
+       assert (¬ (a ∈ [b])).
+       { rewrite /not. intros Hin. apply elem_of_list_singleton in Hin. congruence. }
+       destruct (decide_rel elem_of a [b]); first contradiction.
+       rewrite -minus_n_O /=.
+       inversion Hndup; subst.
+       apply elem_of_cons in Ha.
+       destruct Ha as [Hcontr | Ha]; first congruence.
+       apply IHl1 in Ha as Heq; auto.
+       rewrite Heq. 
+       destruct l1; first inversion Ha. 
+       simpl. lia.
+   Qed.
+
+   Lemma list_difference_app {A : Type} `{EqDecision A}
+         (l1 l2 l2' : list A) :
+     list_difference l1 (l2 ++ l2') = list_difference (list_difference l1 l2) l2'.
+   Proof.
+     induction l1; auto. 
+     simpl. destruct (decide_rel elem_of a (l2 ++ l2')). 
+     - apply elem_of_app in e as [Hl2 | Hl2'].
+       + destruct (decide_rel elem_of a l2); last contradiction.
+         apply IHl1.
+       + destruct (decide_rel elem_of a l2); first by apply IHl1. 
+         simpl.
+         destruct (decide_rel elem_of a l2'); last contradiction.
+         apply IHl1. 
+     - apply not_elem_of_app in n as [Hl2 Hl2']. 
+       destruct (decide_rel elem_of a l2); first contradiction. 
+       simpl.
+       destruct (decide_rel elem_of a l2'); first contradiction. 
+       f_equal. apply IHl1.
+   Qed. 
+
+
+   Ltac discharge_not_or :=
+     rewrite /not; intros Hor;
+       by repeat (destruct Hor as [Hcontr | Hor]; first inversion Hcontr).
+  
+  (* helper lemmas *)
+  Lemma helper1 r1 :
+     r1 ≠ PC ∧ r1 ≠ r_stk ∧ r1 ≠ r_t0 →
+     r1 ∈ all_registers →
+     length (list_difference all_registers [PC; r_stk; r_t0; r1]) = 29.
+   Proof.
+     intros (Hne1 & Hne2 & Hne3) Hr1.
+     assert ([PC; r_stk; r_t0; r1] = [PC; r_stk; r_t0] ++ [r1]); first done. 
+     rewrite H. 
+     rewrite list_difference_app.
+     assert (r1 ∈ (list_difference all_registers [PC; r_stk; r_t0])).
+     { simpl.
+       rewrite /all_registers in Hr1.
+       apply elem_of_cons in Hr1 as [Hcontr | Hr1]; first contradiction.
+       assert 
+       ([r_t1; r_t2; r_t3; r_t4; r_t5; r_t6; r_t7; r_t8; r_t9; r_t10; r_t11;
+          r_t12; r_t13; r_t14; r_t15; r_t16; r_t17; r_t18; r_t19; r_t20; r_t21; r_t22;
+          r_t23; r_t24; r_t25; r_t26; r_t27; r_t28; r_t29; r_t30; r_t31; PC] =
+       [r_t1; r_t2; r_t3; r_t4; r_t5; r_t6; r_t7; r_t8; r_t9; r_t10; r_t11;
+          r_t12; r_t13; r_t14; r_t15; r_t16; r_t17; r_t18; r_t19; r_t20; r_t21; r_t22;
+          r_t23; r_t24; r_t25; r_t26; r_t27; r_t28; r_t29; r_t30] ++ [r_t31; PC]); auto. 
+       rewrite H0 in Hr1. clear H0.
+       apply elem_of_app in Hr1 as [Hr1 | Hcontr]; auto.
+       apply elem_of_cons in Hcontr as [? | Hcontr]; first contradiction.
+       apply elem_of_list_singleton in Hcontr; contradiction. 
+     }
+     rewrite list_difference_length; auto.
+     simpl.
+     repeat (apply NoDup_cons; first discharge_not_or).
+     apply NoDup_nil. 
+   Qed. 
+
+
+   Lemma all_registers_correct r1 :
+     r1 ∈ all_registers.
+   Proof.
+     rewrite /all_registers.
+     destruct r1.
+     - do 32 (apply elem_of_cons; right).
+         by apply elem_of_list_singleton.
+     - induction n.
+       + apply elem_of_cons; left. (* rewrite /r_t0. *)
+         apply f_equal. apply eq_proofs_unicity. decide equality.
+       + apply elem_of_list_lookup_2 with (S n).
+         repeat (destruct n;
+                   first (simpl;do 2 f_equal;apply eq_proofs_unicity;decide equality)).
+         simpl in *. inversion fin.
+   Qed. 
