theories/fundamental.v
@@ -4,7 +4,7 @@ From iris.program_logic Require Import weakestpre adequacy lifting.
 From stdpp Require Import base. 
 
 Section fundamental.
-  Context `{memG Σ, regG Σ, STSG Σ}.
+  Context `{memG Σ, regG Σ, STSG Σ, logrel_na_invs Σ}.
   Notation D := ((leibnizC Word) -n> iProp Σ).
   Notation R := ((leibnizC Reg) -n> iProp Σ).
   Implicit Types w : (leibnizC Word).
@@ -33,52 +33,36 @@ Section fundamental.
     iSpecialize ("Hupdate" with "[Hmap]"); eauto.
   Qed.
 
-  Lemma extract_lookup_reg reg (r : RegName) :
-    ((∀ r0, ⌜is_Some (reg !! r0)⌝ ∧ (⌜r0 ≠ PC⌝ → (fixpoint interp1) (reg !r! r0))) →
-     ⌜is_Some (reg !! r)⌝)%I.
-  Proof.
-    iIntros "Hreg". 
-    - iAssert (⌜is_Some (reg !! r)⌝ ∧ (⌜r ≠ PC⌝ → (fixpoint interp1) (reg !r! r)))%I
-        with "Hreg" as "Hreg". 
-      iDestruct ("Hreg") as "[Hr Hreg]". done. 
-  Qed.
+  Instance addr_inhabited: Inhabited Addr := populate (A 0%Z eq_refl).
 
-  Lemma extract_valid_reg reg (r : RegName) :
-    r ≠ PC →
-    ((∀ r0, ⌜is_Some (reg !! r0)⌝ ∧ (⌜r0 ≠ PC⌝ → (fixpoint interp1) (reg !r! r0))) →
-     (fixpoint interp1) (reg !r! r))%I.
-  Proof.
-    iIntros (Hne) "Hreg".
-    iAssert (⌜is_Some (reg !! r)⌝ ∧ (⌜r ≠ PC⌝ → (fixpoint interp1) (reg !r! r)))%I
-                                             with "Hreg" as "[_ Hv]". 
-    iApply "Hv". iPureIntro. done. 
-  Qed. 
 
-  Instance addr_inhabited: Inhabited Addr := populate (A 0%Z eq_refl). 
-
-  Lemma fundamental_RX b e g (a : Addr) ws :
-    (inv (logN .@ (b,e)) (read_only_cond b e ws interp) →
-     ⟦ inr ((RX,g),b,e,a) ⟧ₑ )%I
-  with fundamental_RWX b e g (a : Addr) :
-    (inv (logN .@ (b,e)) (read_write_cond b e interp) →
-     ⟦ inr ((RWX,g),b,e,a) ⟧ₑ )%I
-  with fundamental_RWLX b e g (a : Addr) :
-    (inv (logN .@ (b,e)) (read_write_local_cond b e interp) →
-     ⟦ inr ((RWLX,g),b,e,a) ⟧ₑ )%I. 
+  Lemma fundamental_RX stsf E r b e g (a : Addr) ws :
+    (na_inv logrel_nais (logN .@ (b,e)) (read_only_cond b e ws stsf E interp) →
+     ⟦ inr ((RX,g),b,e,a) ⟧ₑ stsf E r)%I
+  with fundamental_RWX stsf E r b e g (a : Addr) :
+    (na_inv logrel_nais (logN .@ (b,e)) (read_write_cond b e stsf E interp) →
+     ⟦ inr ((RWX,g),b,e,a) ⟧ₑ stsf E r)%I
+  with fundamental_RWLX stsf E r b e g (a : Addr) :
+    (na_inv logrel_nais (logN .@ (b,e)) (read_write_local_cond b e stsf E interp) →
+     ⟦ inr ((RWLX,g),b,e,a) ⟧ₑ stsf E r)%I. 
   Proof.
-  {
-    iIntros "#Hinv /=".
-    iIntros (r m fs fr) "[Hreg [Hmreg Hsts]]".
+  { destruct stsf as [fs [fr_pub fr_priv] ].
+    iIntros "#Hinv /=". iExists fs,fr_pub,fr_priv.
+    repeat (iSplit;auto). 
+    iIntros "[[Hfull Hreg] [Hmreg [Hsts [Hown #Hreach]]]]".
     iExists _,_,_,_,_; iSplit; eauto; simpl.
-    iRevert "Hinv". iLöb as "IH" forall (r a g fs fr b e ws). iIntros "#Hinv". 
-    iDestruct "Hreg" as "#Hreg". 
+    iRevert "Hinv Hreach". iLöb as "IH" forall (r a g fs fr_priv b e ws).
+    iIntros "#Hinv %". rename a0 into Hreach. 
+    iDestruct "Hfull" as "%". iDestruct "Hreg" as "#Hreg". 
     iApply (wp_bind (fill [SeqCtx])).
     destruct (decide (isCorrectPC (inr ((RX,g),b,e,a)))). 
     - (* Correct PC *)
       assert ((b <= a)%a ∧ (a <= e)%a) as Hbae.
       { eapply in_range_is_correctPC; eauto.
         unfold le_addr; omega. }
-      iInv (logN.@(b, e)) as "Hregion" "Hcls".      
+      iAssert (⌜↑logN.@(b, e) ⊆ E⌝)%I as %Hbe.
+      { iPureIntro. by apply Hreach. }
+      iMod (na_inv_open _ _ _ (logN.@(b, e)) with "Hinv Hown") as "(Hregion & Hown & Hcls)"; auto. 
       iDestruct (extract_from_region _ _ a with "Hregion")
         as (al w ah) "(Hal & Hah & Hregionl & Hvalidl & >Ha & #Hva & Hregionh & Hvalidh)";
         auto.
@@ -96,18 +80,16 @@ Section fundamental.
           iApply wp_pure_step_later; auto.
           iApply wp_value.
           iDestruct (extract_from_region _ _ a with
-               "[Hal Hah Hregionl Hvalidl Hregionh Hvalidh Ha]") as "Hregion"; eauto.
+                         "[Hal Hah Hregionl Hvalidl Hregionh Hvalidh Ha]")
+            as "[Hregion Hvalid]"; eauto.
           { iExists al,w,ah. iFrame. iExact "Hva". }
           iDestruct ((big_sepM_delete _ _ PC) with "[HPC Hmap]") as "Hmap /=".
           apply lookup_insert. rewrite delete_insert_delete. iFrame.
-          rewrite insert_insert.
-          iExists (<[PC:=w]> r),fs,fr. iFrame.
-          iAssert (⌜related_sts fs fs fr fr⌝)%I as "#Hrefl". 
-          { iPureIntro. apply related_sts_refl. }
-          iFrame "#". iApply "Hcls". iNext. iFrame. 
+          iNext. iIntros "%"; inversion a0.
         * (* Load PC src ==> success if src ↦ inr, fail o/w *)
-          iDestruct (extract_lookup_reg r src with "Hreg") as "%".
-          destruct H2 as [wsrc Hsomesrc]. 
+          simpl in H3. 
+          specialize H3 with src as Hsrc. 
+          destruct Hsrc as [wsrc Hsomesrc]. 
           assert ((delete PC r !! src) = Some wsrc) as Hsomesrc'.
           { rewrite -Hsomesrc. apply (lookup_delete_ne r PC src). eauto. }
           rewrite delete_insert_delete.
@@ -118,17 +100,15 @@ Section fundamental.
             iNext. iIntros "[HPC [Ha Hsrc]] /=".
             iApply wp_pure_step_later; auto. iApply wp_value.
             iDestruct (extract_from_region _ _ a with
-                 "[Hal Hah Hregionl Hvalidl Hregionh Hvalidh Ha]") as "Hregion"; eauto.
+                           "[Hal Hah Hregionl Hvalidl Hregionh Hvalidh Ha]")
+              as "[Hregion Hvalid]"; eauto.
             { iExists al,w,ah. iFrame. iExact "Hva". }
             iDestruct ((big_sepM_delete _ _ src) with "[Hsrc Hmap]") as "Hmap /=".
             apply lookup_insert. rewrite delete_insert_delete. iFrame.
             rewrite -delete_insert_ne; auto.
             iDestruct ((big_sepM_delete _ _ PC) with "[HPC Hmap]") as "Hmap /=".
             apply lookup_insert. rewrite delete_insert_delete. iFrame.
-            iExists _,fs,fr. iFrame.
-            iAssert (⌜related_sts fs fs fr fr⌝)%I as "#Hrefl". 
-            { iPureIntro. apply related_sts_refl. }
-            iFrame "#". iApply "Hcls". iNext. iFrame. 
+            iNext. iIntros "%"; inversion a0.  
           } 
           (* src ↦ inr c ==> need to open invariant *)
           destruct c. do 3 destruct p.
@@ -142,38 +122,53 @@ Section fundamental.
               iApply wp_pure_step_later; auto.
               iApply wp_value.
               iDestruct (extract_from_region _ _ a with
-                 "[Hal Hah Hregionl Hvalidl Hregionh Hvalidh Ha]") as "Hregion"; eauto.
+                             "[Hal Hah Hregionl Hvalidl Hregionh Hvalidh Ha]")
+                as "[Hregion Hvalid]"; eauto.
             { iExists al,w,ah. iFrame. iExact "Hva". }
             iDestruct ((big_sepM_delete _ _ src) with "[Hsrc Hmap]") as "Hmap /=".
             apply lookup_insert. rewrite delete_insert_delete. iFrame.
             rewrite -delete_insert_ne; auto.
             iDestruct ((big_sepM_delete _ _ PC) with "[HPC Hmap]") as "Hmap /=".
             apply lookup_insert. rewrite delete_insert_delete. iFrame.
-            iExists _,fs,fr. iFrame.
-            iAssert (⌜related_sts fs fs fr fr⌝)%I as "#Hrefl". 
-            { iPureIntro. apply related_sts_refl. }
-            iFrame "#". iApply "Hcls". iNext. iFrame. 
+            iNext. iIntros "%"; inversion a3. 
           }
           (* readAllowed p && withinBounds ((p,l),a2,a1,a0) *)
           apply (not_false_is_true (_ && _)),Is_true_eq_left,andb_prop_elim in n0
             as [Hra Hwb]. apply andb_prop_elim in Hwb as [Hle Hge]. 
           (* get validity of capability in src from Hreg *)
-          iDestruct (extract_valid_reg r src with "Hreg") as "#Hvsrc"; auto.
+          apply reg_eq_sym in n. 
+          iDestruct ("Hreg" $! src n) as "Hvsrc". 
           rewrite /RegLocate Hsomesrc.
           iDestruct (read_allowed_inv with "Hvsrc") as "Hconds"; eauto.
           (* Each condition in Hconds take a step in similar fashion *)
-          iAssert ((∃ w, (a0 ↦ₐ w -∗
-                   |={⊤ ∖ ↑logN.@(b, e) ∖ ↑logN.@(a2, a1),⊤ ∖ ↑logN.@(b, e)}=> emp)
-            ∗  a0 ↦ₐ w ∗ ▷ ⟦ w ⟧)
-           -∗ WP Instr Executable @ ⊤ ∖ ↑logN.@(b, e) ∖ ↑logN.@(a2, a1)
-                 {{ v, |={⊤ ∖ ↑logN.@(b, e) ∖ ↑logN.@(a2, a1),⊤ ∖ ↑logN.@(b, e)}=>
-                    |={⊤ ∖ ↑logN.@(b, e),⊤}=> WP fill [SeqCtx] (of_val v)
-                    {{ v, (λne _ : valC cap_lang, ∃ r0 fs' fr',
-                          registers_mapsto r0 ∗ ⌜related_sts fs fs' fr fr'⌝
-                                           ∗ sts_full fs' fr') v }} }})%I
-            with "[-]" as "Hstep".
+          rewrite /read_write_cond. 
+          iAssert ((∃ w', ▷ (a0 ↦ₐ w' ∗ a ↦ₐ w
+                   ={⊤}=∗ na_own logrel_nais E)
+            ∗ ▷ a0 ↦ₐ w' ∗ ▷ ▷ ⟦ w' ⟧ E (fs,(fr_pub,fr_priv))
+                   (* ∗ (∃ E', ⌜get_namespace w' = Some E'⌝ ∧ ⌜↑E' ⊆ E⌝)*))
+            ∗ sts_full fs fr_pub fr_priv
+            -∗ WP Instr Executable
+           {{ v, WP fill [SeqCtx] (of_val v)
+                    {{ v0, ⌜v0 = HaltedV⌝
+                      → ∃ (r0 : Reg) (fs' : STS_states) (fr_pub' fr_priv' : STS_rels),
+                           full_map r0
+                           ∧ registers_mapsto r0
+                                              ∗ ⌜related_sts fs fs' fr_priv fr_priv'⌝
+                                              ∗ na_own logrel_nais E
+                                              ∗ sts_full fs' fr_pub' fr_priv' }} }} )%I
+            with "[Ha HPC Hsrc Hmap]" as "Hstep".
           {
-            iIntros "Hw0". iDestruct "Hw0" as (w0) "(Hcls' & Ha0 & #Hw0)". 
+            iIntros "(Hw0 & Hsts)".
+            iDestruct "Hw0" as (w0) "(Hcls' & Ha0 & #Hw0)".
+            (* iDestruct "Hsub" as (E') "#[Hns Hsub]".  *)
+            iAssert (∀ w1 w2, full_map (<[PC:=w1]> (<[src:=w2]> r)))%I as "#Hfull".
+            { iIntros (w1 w2 r0).
+              iPureIntro.
+              destruct (decide (PC = r0)); [simplify_eq; rewrite lookup_insert; eauto|].
+              rewrite lookup_insert_ne.
+              destruct (decide (src = r0)); [simplify_eq; rewrite lookup_insert; eauto|].
+              rewrite lookup_insert_ne. apply H3. done. done.
+            }
             destruct w0.
             { iApply (wp_load_fail5 with "[HPC Ha Hsrc Ha0]"); eauto.
               - split; apply Is_true_eq_true; eauto.
@@ -182,44 +177,19 @@ Section fundamental.
               - iNext. iIntros "[HPC [Ha [Hsrc Ha0]]] /=".
                 iApply wp_pure_step_later; auto.
                 iApply wp_value.
-                iDestruct (extract_from_region _ _ a with
-                  "[Hal Hah Hregionl Hvalidl Hregionh Hvalidh Ha]") as "Hregion"; eauto.
-                { iExists al,w,ah. iFrame. iExact "Hva". }
-                iDestruct ((big_sepM_delete _ _ src) with "[Hsrc Hmap]") as "Hmap /=".
-                apply lookup_insert. rewrite delete_insert_delete. iFrame.
-                rewrite -delete_insert_ne; auto.
-                iDestruct ((big_sepM_delete _ _ PC) with "[HPC Hmap]") as "Hmap /=".
-                apply lookup_insert. rewrite delete_insert_delete. iFrame.
-                iExists _,fs,fr. iFrame.
-                iAssert (⌜related_sts fs fs fr fr⌝)%I as "#Hrefl". 
-                { iPureIntro. apply related_sts_refl. }
-                iFrame "#". iApply "Hcls". iFrame. iApply "Hcls'". iFrame. (* iNext. *)
-                (* iApply (extract_from_region _ _ a0); *)
-                (*   first (split; by apply Z.leb_le,Is_true_eq_true). *)
-                (* iFrame. iExists a0l, (inl z), a0h. iFrame. iExact "Hva0".  *)
+                iNext. iIntros "%"; inversion a3. 
             }
-            destruct c,p0,p0,p0. 
+            destruct c,p0,p0,p0.
             destruct ((a3 + 1)%a) eqn:Ha0.
             2: { (* If src points to top address, load crashes *)
-              iApply (wp_load_fail4 with "[HPC Hsrc Ha Ha0]"); eauto. 
+              iApply (wp_load_fail4 with "[HPC Hsrc Ha Ha0]"); eauto.
               - split; apply Is_true_eq_true; eauto.
                 apply andb_prop_intro. split; [apply Hle|apply Hge].
               - iFrame.
               - iNext. iIntros "[HPC [Ha [Hsrc Ha0]]] /=".
                 iApply wp_pure_step_later; auto.
                 iApply wp_value.
-                iDestruct (extract_from_region _ _ a with
-                  "[Hal Hah Hregionl Hvalidl Hregionh Hvalidh Ha]") as "Hregion"; eauto.
-                { iExists al,w,ah. iFrame. iExact "Hva". }
-                iDestruct ((big_sepM_delete _ _ src) with "[Hsrc Hmap]") as "Hmap /=".
-                apply lookup_insert. rewrite delete_insert_delete. iFrame.
-                rewrite -delete_insert_ne; auto.
-                iDestruct ((big_sepM_delete _ _ PC) with "[HPC Hmap]") as "Hmap /=".
-                apply lookup_insert. rewrite delete_insert_delete. iFrame.
-                iExists _,fs,fr. iFrame.
-                iAssert (⌜related_sts fs fs fr fr⌝)%I as "#Hrefl". 
-                { iPureIntro. apply related_sts_refl. }
-                iFrame "#". iApply "Hcls". iFrame. iApply "Hcls'". iFrame.
+                iNext. iIntros "%"; inversion a6. 
             }
             (* successful load into PC *)
             iApply (wp_load_success_PC with "[HPC Ha Hsrc Ha0]"); eauto.
@@ -228,17 +198,8 @@ Section fundamental.
             - iFrame.
             - iNext. iIntros "[HPC [Ha [Hsrc Ha0]]] /=".
               iApply wp_pure_step_later; auto.
-              (* recontruct regions *)
-              iDestruct (extract_from_region _ _ a with
-                "[Hal Hah Hregionl Hvalidl Hregionh Hvalidh Ha]") as "Hregion"; eauto.
-              { iExists al,w,ah. iFrame. iExact "Hva". }
-              (* We want to apply the IH on the updated r, however the PC has now 
-                 changed region entirely! We have four cases: either the permission 
-                 of the updated PC is valid: i.e. RX (IH), RWX (second lemma), 
-                 RWLX (third lemma), or the permission is not valid, and the program 
-                 crashes *)  
               iAssert (⌜p0 ≠ RX⌝ ∧ ⌜p0 ≠ RWX⌝ ∧ ⌜p0 ≠ RWLX⌝ →
-                       PC ↦ᵣ inr (p0, l0, a5, a4, a6) -∗ 
+                       PC ↦ᵣ inr (p0, l0, a5, a4, a6) -∗
                           WP Seq (Instr Executable) {{ w, ⌜w = FailedV⌝
                                   ∗ PC ↦ᵣ inr (p0, l0, a5, a4, a6) }})%I
                 as "Hfail".
@@ -248,21 +209,22 @@ Section fundamental.
                   [apply not_isCorrectPC_perm; eauto|iFrame|].
                 iNext. iIntros "HPC /=".
                 iApply wp_pure_step_later; auto.
-                iNext. iApply wp_value. iFrame. done. 
+                iNext. iApply wp_value. iFrame. done.
               }
               (* The new register state is valid *)
-              iAssert (interp_registers (<[src:=inr (p, l, a2, a1, a0)]> r)) as "Hreg'".
-              { iIntros (r0). iDestruct ("Hreg" $! (r0)) as "[% Hv]".
-                  destruct H2 as [c Hsome].
-                  iSplit; auto.
-                - iPureIntro.
+              iAssert (interp_registers _ _ (<[src:=inr (p, l, a2, a1, a0)]> r)) as "[Hfull' Hreg']".
+              { iSplitL.
+                { iIntros (r0). iPureIntro.
                   destruct (decide (src = r0)); simplify_eq;
-                    [rewrite lookup_insert|rewrite lookup_insert_ne]; eauto. 
-                - iIntros (Hnepc) "/=".
-                  destruct (decide (src = r0)); simplify_eq.
+                    [rewrite lookup_insert|rewrite lookup_insert_ne]; eauto. }
+                iIntros (r0) "%".
+                destruct (decide (src = r0)); simplify_eq.
                   + by rewrite /RegLocate lookup_insert.
-                  + rewrite /RegLocate lookup_insert_ne; auto. 
-                    rewrite Hsome. iApply "Hv"; auto.  
+                  + rewrite /RegLocate lookup_insert_ne; auto.
+                    iDestruct ("Hreg" $! (r0) a7) as "Hr0".
+                    specialize H3 with r0.
+                    destruct H3 as [c Hsome].
+                    rewrite Hsome. iApply "Hr0"; auto.
               }
               destruct p0;
                 [iAssert (⌜O ≠ RX⌝ ∧ ⌜O ≠ RWX⌝ ∧ ⌜O ≠ RWLX⌝)%I as "Htrivial";
@@ -273,30 +235,30 @@ Section fundamental.
                  first (iSplit; iPureIntro; auto)|
                  iAssert (⌜RWL ≠ RX⌝ ∧ ⌜RWL ≠ RWX⌝ ∧ ⌜RWL ≠ RWLX⌝)%I as "Htrivial";
                  first (iSplit; iPureIntro; auto)| |
-                 iAssert (⌜E ≠ RX⌝ ∧ ⌜E ≠ RWX⌝ ∧ ⌜E ≠ RWLX⌝)%I as "Htrivial";
+                 iAssert (⌜cap_lang.E ≠ RX⌝ ∧ ⌜cap_lang.E ≠ RWX⌝ ∧ ⌜cap_lang.E ≠ RWLX⌝)%I as "Htrivial";
                  first (iSplit; iPureIntro; auto)| | ];
-              try ( iDestruct ("Hfail" with "Htrivial HPC") as "Hfail";
-                    iApply (wp_wand with "Hfail");
-                    iAssert ((∀ v : val cap_lang, ⌜v = FailedV⌝
-                                ∗ PC ↦ᵣ inr (_, l0, a5, a4, a6)
-                               -∗ ∃ (r0 : Reg) (fs' : STS_states) (fr' : STS_rels),
-                               registers_mapsto r0 ∗ ⌜related_sts fs fs' fr fr'⌝
-                                                ∗ sts_full fs' fr'))%I
-                      with "[Hmap Hsrc Hsts]" as "Hfailed";
-                    [ iIntros (v) "[-> HPC]";
-                      iDestruct ((big_sepM_delete _ _ src)
-                                   with "[Hsrc Hmap]") as "Hmap /=";
-                      [apply lookup_insert|rewrite delete_insert_delete;iFrame|];
-                      rewrite -delete_insert_ne; auto;
-                      iDestruct ((big_sepM_delete _ _ PC)
-                                   with "[HPC Hmap]") as "Hmap /=";
-                      [apply lookup_insert|rewrite delete_insert_delete;iFrame|];
-                      iExists _,fs,fr; iFrame; iPureIntro; apply related_sts_refl
-                     |];
-                    iFrame;
-                    (* close invariants *)
-                    iApply "Hcls"; iFrame; iApply "Hcls'"; iFrame
-                  ).
+                try ( iDestruct ("Hfail" with "Htrivial HPC") as "Hfail";
+                      iApply (wp_wand with "Hfail");
+                        iAssert ((∀ v : val cap_lang, ⌜v = FailedV⌝
+                               ∗ PC ↦ᵣ inr (_, l0, a5, a4, a6)
+                               -∗ ⌜v = HaltedV⌝
+                                  → ∃ (r0 : Reg) fs' fr_pub' fr_priv',
+                                       full_map r0 ∧ registers_mapsto r0 ∗ ⌜related_sts fs fs' fr_priv fr_priv'⌝
+                                                                      ∗ na_own logrel_nais E
+                                                                      ∗ sts_full fs' fr_pub' fr_priv'))%I
+                  with "[Hmap Hsrc Hsts]" as "Hfailed";
+                [ iIntros (v) "[-> HPC]";
+                  iDestruct ((big_sepM_delete _ _ src)
+                               with "[Hsrc Hmap]") as "Hmap /=";
+                  [apply lookup_insert|rewrite delete_insert_delete;iFrame|];
+                  rewrite -delete_insert_ne; auto;
+                  iDestruct ((big_sepM_delete _ _ PC)
+                               with "[HPC Hmap]") as "Hmap /=";
+                  [apply lookup_insert|rewrite delete_insert_delete;iFrame|];
+                  iIntros "%"; inversion a7
+                 |];iFrame);
+                try (iNext;iDestruct ("Hfail" with "Htrivial HPC") as "Hfail"; 
+                iApply wp_wand_l;iFrame;iIntros (v) "[-> HPC] %";inversion a7).
               { (* new PC is RX ==> apply IH*)
                 iClear "Hfail".
                 iDestruct ((big_sepM_delete _ _ src) with "[Hsrc Hmap]") as "Hmap /=";
@@ -305,13 +267,16 @@ Section fundamental.
                      iDestruct ((big_sepM_delete _ _ PC) with "[HPC Hmap]") as "Hmap /=";
                      [apply lookup_insert|rewrite delete_insert_delete;iFrame|].
                 (* apply IH *)
-                rewrite (fixpoint_interp1_eq (inr (RX, l0, a5, a4, a3))). simpl.
-                iDestruct "Hw0" as (p0 g0 b0 e0 a7 ws1) "[% [Hb0e0 Hexec]]"; simplify_eq.
-                iApply ("IH" $! _ _ _ _ _ _ _ ws1 with "Hreg' Hmap Hsts").
-                iFrame "Hb0e0".
-                (* reestablish invariants *)
-                iApply "Hcls"; iFrame; iApply "Hcls'"; iFrame.
-              }
+                iNext.
+                rewrite (fixpoint_interp1_eq _ _ (inr (RX, l0, a5, a4, a3))) /=.
+                iDestruct "Hw0" as (p0 g0 b0 e0 a7 ws1) "(% & % & Hb0e0 & Hexec)".
+                inversion H4;subst.
+                iMod ("Hcls'" with "[$Ha0 $Ha]") as "Hown". 
+                iApply ("IH" $! _ _ _ _ _ _ _ ws1
+                          with "[Hfull'] [Hreg'] [Hmap] [Hsts] [Hown]");
+                  iFrame; iFrame "#".
+                iAlways. iPureIntro. by intros ns Hns; inversion Hns.  
+              } 
               { (* new PC is RWX, apply fundamental_RWX *)
                 iClear "Hfail".
                 iDestruct ((big_sepM_delete _ _ src) with "[Hsrc Hmap]") as "Hmap /=";
@@ -319,14 +284,19 @@ Section fundamental.
                      rewrite -delete_insert_ne; auto;
                      iDestruct ((big_sepM_delete _ _ PC) with "[HPC Hmap]") as "Hmap /=";
                      [apply lookup_insert|rewrite delete_insert_delete;iFrame|].
-                rewrite (fixpoint_interp1_eq (inr (RWX, l0, a5, a4, a3))). simpl.
-                iDestruct "Hw0" as (p0 g0 b0 e0 a7) "[% [Hb0e0 Hexec]]"; simplify_eq.
-                iDestruct (fundamental_RWX with "Hb0e0") as "Hexpr". 
-                iDestruct ("Hexpr" $! (<[src:=inr (p, l, a2, a1, a0)]> r) m fs fr
-                             with "[$]")
-                  as (p0 g1 b1 e1 a3) "[% Ho]"; simplify_eq. iFrame.
-                (* reestablish invariants *)
-                iApply "Hcls"; iFrame; iApply "Hcls'"; iFrame.
+                iNext.
+                rewrite (fixpoint_interp1_eq _ _ (inr (RWX, l0, a5, a4, a3))) /=.
+                iDestruct "Hw0" as (p0 g0 b0 e0 a7) "(% & % & Hb0e0 & Hexec)".
+                inversion H4;subst.
+                iMod ("Hcls'" with "[$Ha0 $Ha]") as "Hown". 
+                iDestruct (fundamental_RWX _ _ (<[src:=inr (p, l, a2, a1, a0)]> r)
+                             with "Hb0e0") as "Hexpr"; eauto.
+                iDestruct "Hexpr" as (fs0 frpub0 frpriv0) "(% & % & % & Hexpr)";
+                  simplify_eq.
+                iDestruct ("Hexpr" 
+                             with "[Hfull' Hreg' Hmap Hsts Hown]")
+                  as (p0 g1 b1 e1 a3) "[% Ho]"; simplify_eq; iFrame. 
+                iPureIntro. by intros ns Hns; inversion Hns.  
               }
               { (* new PC is RWLX, apply fundamental_RWLX *)
                 iClear "Hfail".
@@ -335,84 +305,137 @@ Section fundamental.
                      rewrite -delete_insert_ne; auto;
                      iDestruct ((big_sepM_delete _ _ PC) with "[HPC Hmap]") as "Hmap /=";
                      [apply lookup_insert|rewrite delete_insert_delete;iFrame|].
-                rewrite (fixpoint_interp1_eq (inr (RWLX, l0, a5, a4, a3))). simpl.
-                iDestruct "Hw0" as (p0 g0 b0 e0 a7) "[% [Hb0e0 Hexec]]"; simplify_eq.
-                iDestruct (fundamental_RWLX with "Hb0e0") as "Hexpr". 
-                iDestruct ("Hexpr" $! (<[src:=inr (p, l, a2, a1, a0)]> r) m fs fr
-                             with "[$]")
-                  as (p0 g1 b1 e1 a3) "[% Ho]"; simplify_eq. iFrame.
-                (* reestablish invariants *)
-                iApply "Hcls"; iFrame. iApply "Hcls'"; iFrame.
+                rewrite (fixpoint_interp1_eq _ _ (inr (RWLX, l0, a5, a4, a3))).
+                iNext.
+                iDestruct "Hw0" as (p0 g0 b0 e0 a7) "(% & % & Hb0e0 & Hexec)".
+                inversion H4;subst.
+                iMod ("Hcls'" with "[$Ha0 $Ha]") as "Hown". 
+                iDestruct (fundamental_RWLX _ _ (<[src:=inr (p, l, a2, a1, a0)]> r)
+                             with "Hb0e0") as "Hexpr"; eauto.
+                iDestruct "Hexpr" as (fs0 frpub0 frpriv0) "(% & % & % & Hexpr)";
+                  simplify_eq.
+                iDestruct ("Hexpr" 
+                             with "[Hfull' Hreg' Hmap Hsts Hown]")
+                  as (p0 g1 b1 e1 a3) "[% Ho]"; simplify_eq; iFrame.
+                iPureIntro. by intros ns Hns; inversion Hns.  
               }
           }
-          iDestruct "Hconds" as "[#Hro|#[Hrw|Hrwl]]".
+
+          destruct (decide ((b,e) = (a2,a1))).
+          {
+            inversion e0; subst.
+            (* no need to open any invariant, in this case we need to do cases on 
+               a = a0. if a = a0, then the program should crash, since we will not 
+               be able to increment w once loaded into PC. Otherwise we just do as 
+               below, except we don't need to open the invariant, we just destruct the 
+               region a0 is in (either in Hregionl or Hregionh). *)
+            admit. 
+          }
+          iDestruct "Hconds" as "[[#Hro|#[Hrw|Hrwl]] %]".
           (* each condition is similar, but with some subtle differences for closing *)
           { iDestruct "Hro" as (ws0) "Hinv0".
             (* open the invariant to access a0 ↦ₐ _ *)
-            iInv (logN.@(a2, a1)) as "Hro_cond" "Hcls'";[admit|].
+            iMod (na_inv_open _ _ _ (logN.@(a2, a1)) with "Hinv0 Hown")
+              as "(Hro_cond & Hown & Hcls')"; auto.
+            { apply namespace_subseteq_difference; auto.
+              rewrite /namespace_subseteq_difference.
+              by apply ndot_ne_disjoint. 
+            }
+            rewrite /read_only_cond.
             iDestruct (extract_from_region _ _ a0 with "Hro_cond")
-            as (a0l w0 a0h)
-            "(Ha0l & Ha0h & Hregion0l & Hvalid0l & >Ha0 & #Hva0 & Hregion0h & Hvalid0h)";
+              as (a0l w0 a0h)
+                   "(Ha0l & Ha0h & Hregion0l & Hvalid0l & >Ha0 & #Hva0 & Hregion0h & Hvalid0h)";
               first (split; by apply Z.leb_le,Is_true_eq_true).
-            iApply "Hstep".
-            iExists w0. iFrame "Ha0 #". iIntros "Ha0".
-            iApply "Hcls'". iNext.
-            iApply (extract_from_region _ _ a0);
+            iApply "Hstep". iFrame "Hsts".
+            iExists w0. iFrame "Ha0 Hva0". 
+            iNext. iIntros "[Ha0 Ha]".
+            iDestruct (extract_from_region _ _ a0
+                         with "[Hregion0l Hvalid0l Hregion0h Hvalid0h Ha0 Ha0l Ha0h]")
+              as "Hregion";
               first (split; by apply Z.leb_le,Is_true_eq_true).
-            iFrame. iExists a0l, _, a0h. iFrame. iExact "Hva0".
+            { iFrame. iExists a0l, _, a0h. iFrame. iExact "Hva0". }
+            iMod ("Hcls'" with "[$Hown $Hregion]") as "Hown".
+            iDestruct (extract_from_region _ _ a
+                         with "[Hregionl Hvalidl Hregionh Hvalidh Ha Hal Hah]")
+              as "Hregion"; eauto. 
+            { iFrame. iExists al, _, ah. iFrame. iExact "Hva". }
+            iMod ("Hcls" with "[$Hown $Hregion]") as "Hown".
+            iModIntro. iFrame. 
           }
           { (* open the invariant to access a0 ↦ₐ _ *)
-            iInv (logN.@(a2, a1)) as "Hrw_cond" "Hcls'";[admit|].
-            iDestruct "Hrw_cond" as (ws0) "Hrw_cond". 
+            iMod (na_inv_open _ _ _ (logN.@(a2, a1)) with "Hrw Hown")
+              as "(Hrw_cond & Hown & Hcls')"; auto.
+            { apply namespace_subseteq_difference; auto.
+              rewrite /namespace_subseteq_difference.
+              by apply ndot_ne_disjoint. 
+            }
+            rewrite /read_only_cond.
+            iDestruct "Hrw_cond" as (ws0) "Hrw_cond".
             iDestruct (extract_from_region _ _ a0 with "Hrw_cond")
             as (a0l w0 a0h)
      "(Ha0l & Ha0h & Hregion0l & Hvalid0l & >Ha0 & #[Hva0 Hnl] & Hregion0h & Hvalid0h)";
               first (split; by apply Z.leb_le,Is_true_eq_true).
-            iApply "Hstep".
-            iExists w0. iFrame "Ha0 #". iIntros "Ha0".
-            iApply "Hcls'". iNext.
-            iDestruct (extract_from_region _ _ a0 with
-                "[Ha0l Ha0h Hregion0l Hvalid0l Hregion0h Hvalid0h Ha0]") as "Hregion0".
-            { split; apply Z.leb_le,Is_true_eq_true; eauto. }
-            { iExists a0l,_,a0h. iFrame. iFrame "#". }
-            iExists ws0. iFrame.
+            iApply "Hstep". iFrame. 
+            iExists w0. iFrame "Ha0 #".
+            iNext. iIntros "[Ha0 Ha]". 
+            iDestruct (extract_from_region _ _ a0
+                         with "[Hregion0l Hvalid0l Hregion0h Hvalid0h Ha0 Ha0l Ha0h]")
+              as "[Hbe Hregion]";
+              first (split; by apply Z.leb_le,Is_true_eq_true).
+            { iFrame. iExists a0l, _, a0h. iFrame. iFrame "#". } 
+            iMod ("Hcls'" with "[$Hown Hbe Hregion]") as "Hown".
+            { iNext. iExists _. iFrame. iApply big_sepL_later. iNext. iFrame. }
+            iDestruct (extract_from_region _ _ a
+                         with "[Hregionl Hvalidl Hregionh Hvalidh Ha Hal Hah]")
+              as "Hregion"; eauto. 
+            { iFrame. iExists al, _, ah. iFrame. iExact "Hva". }
+            iMod ("Hcls" with "[$Hown $Hregion]") as "Hown".
+            iModIntro. iFrame. 
           }
           { (* open the invariant to access a0 ↦ₐ _ *)
-            iInv (logN.@(a2, a1)) as "Hrw_cond" "Hcls'";[admit|].
-            iDestruct "Hrw_cond" as (ws0) "Hrw_cond". 
-            iDestruct (extract_from_region _ _ a0 with "Hrw_cond")
+            iMod (na_inv_open _ _ _ (logN.@(a2, a1)) with "Hrwl Hown")
+              as "(Hrwl_cond & Hown & Hcls')"; auto.
+            { apply namespace_subseteq_difference; auto.
+              rewrite /namespace_subseteq_difference.
+              by apply ndot_ne_disjoint. 
+            }
+            rewrite /read_only_cond.
+            iDestruct "Hrwl_cond" as (ws0) "Hrwl_cond".
+            iDestruct (extract_from_region _ _ a0 with "Hrwl_cond")
             as (a0l w0 a0h)
-            "(Ha0l & Ha0h & Hregion0l & Hvalid0l & >Ha0 & #Hva0 & Hregion0h & Hvalid0h)";
+     "(Ha0l & Ha0h & Hregion0l & Hvalid0l & >Ha0 & #Hva0 & Hregion0h & Hvalid0h)";
               first (split; by apply Z.leb_le,Is_true_eq_true).
-            iApply "Hstep".
-            iExists w0. iFrame "Ha0 #". iIntros "Ha0".
-            iApply "Hcls'". iNext.
-            iDestruct (extract_from_region _ _ a0 with
-                "[Ha0l Ha0h Hregion0l Hvalid0l Hregion0h Hvalid0h Ha0]") as "Hregion0".
-            { split; apply Z.leb_le,Is_true_eq_true; eauto. }
-            { iExists a0l,_,a0h. iFrame. iFrame "#". }
-            iExists ws0. iFrame. }
-        * iDestruct (extract_lookup_reg r dst with "Hreg") as "%".
-          destruct H2 as [wdst Hsomedst]. 
+            iApply "Hstep". iFrame. 
+            iExists w0. iFrame "Ha0 #".
+            iNext. iIntros "[Ha0 Ha]". 
+            iDestruct (extract_from_region _ _ a0
+                         with "[Hregion0l Hvalid0l Hregion0h Hvalid0h Ha0 Ha0l Ha0h]")
+              as "[Hbe Hregion]";
+              first (split; by apply Z.leb_le,Is_true_eq_true).
+            { iFrame. iExists a0l, _, a0h. iFrame. iFrame "#". } 
+            iMod ("Hcls'" with "[$Hown Hbe Hregion]") as "Hown".
+            { iNext. iExists _. iFrame. iApply big_sepL_later. iNext. iFrame. }
+            iDestruct (extract_from_region _ _ a
+                         with "[Hregionl Hvalidl Hregionh Hvalidh Ha Hal Hah]")
+              as "Hregion"; eauto. 
+            { iFrame. iExists al, _, ah. iFrame. iExact "Hva". }
+            iMod ("Hcls" with "[$Hown $Hregion]") as "Hown".
+            iModIntro. iFrame. 
+          }
+        * destruct (H3 dst) as [wdst Hsomedst].  
           assert ((delete PC r !! dst) = Some wdst) as Hsomedst'.
           { rewrite -Hsomedst. apply (lookup_delete_ne r PC dst). eauto. }
           rewrite delete_insert_delete.
           iDestruct ((big_sepM_delete _ _ dst) with "Hmap") as "[Hdst Hmap]"; eauto. 
           destruct (a + 1)%a eqn:Ha'. 
-          2: (* if PC cannot be incremented ==> dst is updated, then program crashes *)
-            { iApply (wp_load_fail6 with "[HPC Hdst Ha]"); eauto.
+          2: { (* if PC cannot be incremented ==> dst is updated, then program crashes *)
+              iApply (wp_load_fail6 with "[HPC Hdst Ha]"); eauto.
               iFrame. iNext. iIntros "[HPC [Ha Hdst]] /=".
               iApply wp_pure_step_later; auto.
-              iApply wp_value. iExists _,fs,fr. iFrame. 
-              iAssert (⌜related_sts fs fs fr fr⌝)%I as "#Hrefl". 
-              { iPureIntro. apply related_sts_refl. }
-              iFrame "#".
-              iApply "Hcls".
-              iDestruct (extract_from_region _ _ a with
-                  "[Hal Hah Hregionl Hvalidl Hregionh Hvalidh Ha]") as "Hregion"; eauto.
-              iExists _,_,_. iFrame. iDestruct "Hah" as "%".
-              destruct H2 as [Hcontr | ->]; try congruence.
-              iFrame "#". iRight. done. }
+              iApply wp_value; auto.
+              iNext. 
+              iIntros (Hcontr); inversion Hcontr. 
+            }
             (* if PC can be incremented, load succeeds ==> apply IH *)
             iApply (wp_load_success_fromPC with "[HPC Hdst Ha]"); eauto.
             iFrame.
@@ -425,28 +448,31 @@ Section fundamental.
                      iDestruct ((big_sepM_delete _ _ PC) with "[HPC Hmap]") as "Hmap /=";
                      [apply lookup_insert|rewrite delete_insert_delete;iFrame|].
             (* apply IH *)
-            iAssert (interp_registers (<[dst:=w]> r)) as "Hreg'".
-            { iIntros (r0). iDestruct ("Hreg" $! (r0)) as "[% Hv]".
-              destruct H2 as [c Hsome].
-              iSplit; auto.
-              - iPureIntro.
+            iAssert (▷ interp_registers _ (fs, (fr_pub, fr_priv)) (<[dst:=w]> r))%I
+              as "[Hfull Hreg']".
+            { iNext. iSplitL.
+              { iIntros (r0). iPureIntro.
                 destruct (decide (dst = r0)); simplify_eq;
-                    [rewrite lookup_insert|rewrite lookup_insert_ne]; eauto. 
-              - iIntros (Hnepc) "/=".
-                destruct (decide (dst = r0)); simplify_eq.
-                + by rewrite /RegLocate lookup_insert.
-                + rewrite /RegLocate lookup_insert_ne; auto. 
-                  rewrite Hsome. iApply "Hv"; auto.  
+                  [rewrite lookup_insert|rewrite lookup_insert_ne]; eauto. }
+              iIntros (r0) "%".
+              destruct (decide (dst = r0)); simplify_eq.
+                  + by rewrite /RegLocate lookup_insert.
+                  + rewrite /RegLocate lookup_insert_ne; auto.
+                    iDestruct ("Hreg" $! (r0) a1) as "Hr0".
+                    specialize H3 with r0. 
+                    destruct H3 as [c Hsome].
+                    rewrite Hsome. iApply "Hr0"; auto.
             }
-            iApply ("IH" with "Hreg' Hmap Hsts").
-            iFrame "Hinv".
-            (* reestablish invariants *)
-            iApply "Hcls"; iFrame.
+            iNext.
             iDestruct (extract_from_region _ _ a with
-                 "[Hal Hah Hregionl Hvalidl Hregionh Hvalidh Ha]") as "Hregion"; eauto.
-            iExists _,_,_; rewrite Ha'; iFrame. iExact "Hva".
-        * iDestruct (extract_lookup_reg r src with "Hreg") as "%".
-          destruct H2 as [wsrc Hsomesrc].
+                           "[Hal Hah Hregionl Hvalidl Hregionh Hvalidh Ha]")
+              as "[Hbe Hregion]"; eauto.
+            iExists _,_,_; rewrite Ha'; iFrame. iExact "Hva". 
+            iMod ("Hcls" with "[Hbe Hregion $Hown]") as "Hown".
+            { iNext. iFrame. iApply big_sepL_later. iNext. iFrame. }
+            iApply ("IH" with "Hfull Hreg' Hmap Hsts Hown").
+            iExact "Hinv". auto. 
+        * destruct (H3 src) as [wsrc Hsomesrc].
           assert ((delete PC r !! src) = Some wsrc) as Hsomesrc'.
           { rewrite -Hsomesrc. apply (lookup_delete_ne r PC src). eauto. }
           rewrite delete_insert_delete. 
@@ -456,18 +482,7 @@ Section fundamental.
             iApply (wp_load_fail2 with "[HPC Ha Hsrc]"); eauto; iFrame.
             iNext. iIntros "[HPC [Ha Hsrc]] /=".
             iApply wp_pure_step_later; auto. iApply wp_value.
-            iDestruct (extract_from_region _ _ a with
-                 "[Hal Hah Hregionl Hvalidl Hregionh Hvalidh Ha]") as "Hregion"; eauto.
-            { iExists al,w,ah. iFrame. iExact "Hva". }
-            iDestruct ((big_sepM_delete _ _ src) with "[Hsrc Hmap]") as "Hmap /=".
-            apply lookup_insert. rewrite delete_insert_delete. iFrame.
-            rewrite -delete_insert_ne; auto.
-            iDestruct ((big_sepM_delete _ _ PC) with "[HPC Hmap]") as "Hmap /=".
-            apply lookup_insert. rewrite delete_insert_delete. iFrame.
-            iExists _,fs,fr. iFrame.
-            iAssert (⌜related_sts fs fs fr fr⌝)%I as "#Hrefl". 
-            { iPureIntro. apply related_sts_refl. }
-            iFrame "#". iApply "Hcls". iNext. iFrame. 
+            iNext. iIntros (Hcontr); inversion Hcontr. 
           } 
           (* src ↦ inr c ==> need to open invariant *)
           destruct c. do 3 destruct p.
@@ -479,40 +494,34 @@ Section fundamental.
             - iFrame.
             - iNext. iIntros "[HPC [Ha Hsrc]] /=".
               iApply wp_pure_step_later; auto.
-              iApply wp_value.
-              iDestruct (extract_from_region _ _ a with
-                 "[Hal Hah Hregionl Hvalidl Hregionh Hvalidh Ha]") as "Hregion"; eauto.
-            { iExists al,w,ah. iFrame. iExact "Hva". }
-            iDestruct ((big_sepM_delete _ _ src) with "[Hsrc Hmap]") as "Hmap /=".
-            apply lookup_insert. rewrite delete_insert_delete. iFrame.
-            rewrite -delete_insert_ne; auto.
-            iDestruct ((big_sepM_delete _ _ PC) with "[HPC Hmap]") as "Hmap /=".
-            apply lookup_insert. rewrite delete_insert_delete. iFrame.
-            iExists _,fs,fr. iFrame.
-            iAssert (⌜related_sts fs fs fr fr⌝)%I as "#Hrefl". 
-            { iPureIntro. apply related_sts_refl. }
-            iFrame "#". iApply "Hcls". iNext. iFrame. 
+              iApply wp_value. iNext.
+              iIntros (Hcontr); inversion Hcontr. 
           }
           (* readAllowed p && withinBounds ((p,l),a2,a1,a0) *)
           apply (not_false_is_true (_ && _)),Is_true_eq_left,andb_prop_elim in n1
             as [Hra Hwb]. apply andb_prop_elim in Hwb as [Hle Hge].
           (* the contents of src is valid *)
-          iAssert ((fixpoint interp1) (inr (p, l, a2, a1, a0))) as "#Hvsrc".
-          { iDestruct ("Hreg" $! src) as "[_ Hvsrc]".
+          iAssert ((fixpoint interp1) _ _ (inr (p, l, a2, a1, a0))) as "#Hvsrc".
+          { apply reg_eq_sym in n0. iDestruct ("Hreg" $! src n0) as "Hvsrc".
             rewrite /RegLocate Hsomesrc /=. by iApply "Hvsrc". }
           iDestruct (read_allowed_inv with "Hvsrc") as "Hconds"; eauto.
           (* Each condition in Hconds take a step in similar fashion *)
-          iAssert ((∃ w, (a0 ↦ₐ w -∗
-                   |={⊤ ∖ ↑logN.@(b, e) ∖ ↑logN.@(a2, a1),⊤ ∖ ↑logN.@(b, e)}=> emp)
-            ∗  a0 ↦ₐ w ∗ ▷ ⟦ w ⟧)
-           -∗ WP Instr Executable @ ⊤ ∖ ↑logN.@(b, e) ∖ ↑logN.@(a2, a1)
-                 {{ v, |={⊤ ∖ ↑logN.@(b, e) ∖ ↑logN.@(a2, a1),⊤ ∖ ↑logN.@(b, e)}=>
-                    |={⊤ ∖ ↑logN.@(b, e),⊤}=> WP fill [SeqCtx] (of_val v)
-                    {{ v, (λne _ : valC cap_lang, ∃ r0 fs' fr',
-                          registers_mapsto r0 ∗ ⌜related_sts fs fs' fr fr'⌝
-                                           ∗ sts_full fs' fr') v }} }})%I
-            with "[-]" as "Hstep".
-          { iIntros "Hcls'". iDestruct "Hcls'" as (w0) "[Hcls' [Ha0 #Hw0]]". 
+          iAssert ((∃ w', ▷ (a0 ↦ₐ w' ∗ a ↦ₐ w
+                   ={⊤}=∗ na_own logrel_nais E)
+            ∗ ▷ a0 ↦ₐ w' ∗ ▷ ▷ ⟦ w' ⟧ E (fs,(fr_pub,fr_priv))
+                   (* ∗ (∃ E', ⌜get_namespace w' = Some E'⌝ ∧ ⌜↑E' ⊆ E⌝)*))
+            ∗ sts_full fs fr_pub fr_priv
+            -∗ WP Instr Executable
+           {{ v, WP fill [SeqCtx] (of_val v)
+                    {{ v0, ⌜v0 = HaltedV⌝
+                      → ∃ (r0 : Reg) (fs' : STS_states) (fr_pub' fr_priv' : STS_rels),
+                           full_map r0
+                           ∧ registers_mapsto r0
+                                              ∗ ⌜related_sts fs fs' fr_priv fr_priv'⌝
+                                              ∗ na_own logrel_nais E
+                                              ∗ sts_full fs' fr_pub' fr_priv' }} }} )%I
+            with "[Ha HPC Hsrc Hmap]" as "Hstep".
+          { iIntros "[Hcls' Hsts]". iDestruct "Hcls'" as (w0) "[Hcls' [Ha0 #Hw0]]". 
             (* if PC cannot be incremented ==> dst is updated, then program crashes *)
             destruct (a + 1)%a eqn:Ha'; simplify_eq.
             2: { destruct (decide (src = dst)); simplify_eq. 
@@ -520,16 +529,9 @@ Section fundamental.
                    { split; apply Is_true_eq_true; eauto. apply andb_prop_intro. eauto. }
                    iFrame. iNext. iIntros "[HPC [Ha [Hdst Ha0]]] /=".
                    iApply wp_pure_step_later; auto.
-                   iApply wp_value. iExists _,fs,fr. iFrame. 
-                   iAssert (⌜related_sts fs fs fr fr⌝)%I as "#Hrefl". 
-                   { iPureIntro. apply related_sts_refl. }
-                   iFrame "#". iApply "Hcls".
-                   iDestruct (extract_from_region _ _ a with
-                  "[Hal Hah Hregionl Hvalidl Hregionh Hvalidh Ha]") as "Hregion"; eauto.
-                   iExists _,_,_; rewrite Ha'; iFrame "∗ #". iFrame.
-                   iApply "Hcls'". iFrame.
-                 - iDestruct (extract_lookup_reg r dst with "Hreg") as "%".
-                   destruct H2 as [wdst Hsomedst].
+                   iApply wp_value. iNext.
+                   iIntros (Hcontr); inversion Hcontr. 
+                 - destruct (H3 dst) as [wdst Hsomedst].
                    assert (delete PC r !! dst = Some wdst) as Hsomedst'.
                    { rewrite -Hsomedst. apply (lookup_delete_ne r PC dst). eauto. }
                    assert (delete src (delete PC r) !! dst = Some wdst) as Hsomedst''.
@@ -541,15 +543,9 @@ Section fundamental.
                    { split; apply Is_true_eq_true; eauto. apply andb_prop_intro. eauto. }
                    iFrame. iNext. iIntros "(HPC & Ha & Hsrc & Ha0 & Hdst) /=".
                    iApply wp_pure_step_later; auto.
-                   iApply wp_value. iExists _,fs,fr. iFrame. 
-                   iAssert (⌜related_sts fs fs fr fr⌝)%I as "#Hrefl". 
-                   { iPureIntro. apply related_sts_refl. }
-                   iFrame "#". iApply "Hcls".
-                   iDestruct (extract_from_region _ _ a with
-                  "[Hal Hah Hregionl Hvalidl Hregionh Hvalidh Ha]") as "Hregion"; eauto.
-                   iExists _,_,_; rewrite Ha'; iFrame "∗ #". iFrame.
-                   iApply "Hcls'". iFrame.
-            }
+                   iApply wp_value. iNext.
+                   iIntros (Hcontr); inversion Hcontr. 
+                }
             (* two successful steps: loading to a fresh dst, and loading to src *)
             destruct (decide (src = dst)); simplify_eq.
             - iApply (wp_load_success_same with "[HPC Hsrc Ha Ha0]"); eauto.
@@ -564,29 +560,25 @@ Section fundamental.
               (* apply IH *)
               (* we will apply the IH on an updated register state *)
               (* we can only prove the following once we have taken a step *)
-              iAssert (interp_registers (<[dst:=w0]> r)) as "Hreg'".
-              { iIntros (r0). iDestruct ("Hreg" $! (r0)) as "[% Hv]".
-                destruct H2 as [c Hsome].
-                iSplit; auto.
-                - iPureIntro.
+              iAssert (▷ interp_registers _ _ (<[dst:=w0]> r))%I as "[Hfull' Hreg']".
+              { iNext. iSplitR.
+                - iIntros (r0).
+                  iPureIntro.
+                  destruct (H3 r0) as [c Hsome]. 
                   destruct (decide (dst = r0)); simplify_eq;
-                    [rewrite lookup_insert|rewrite lookup_insert_ne]; eauto. 
-                - iIntros (Hnepc) "/=".
+                    [rewrite lookup_insert|rewrite lookup_insert_ne]; eauto.
+                - iIntros (r0) "% /=".
+                  iDestruct ("Hreg" $! (r0)) as "Hv".
+                  destruct (H3 r0) as [c Hsome]. 
                   destruct (decide (dst = r0)); simplify_eq.
                   + rewrite /RegLocate lookup_insert. iApply "Hw0". 
                   + rewrite /RegLocate lookup_insert_ne; auto. 
                     rewrite Hsome. iApply "Hv"; auto.  
               }
-              iApply ("IH" with "Hreg' Hmap Hsts").
-              iFrame "Hinv".
-              (* reestablish invariants *)
-              iApply "Hcls"; iFrame.
-              iDestruct (extract_from_region _ _ a with
-                "[Hal Hah Hregionl Hvalidl Hregionh Hvalidh Ha]") as "Hregion"; eauto.
-              iExists _,_,_; rewrite Ha'; iFrame. iExact "Hva". iFrame. 
-              iApply "Hcls'". iFrame. 
-            - iDestruct (extract_lookup_reg r dst with "Hreg") as "%".
-              destruct H2 as [wdst Hsomedst].
+              iNext.
+              iMod ("Hcls'" with "[$Ha0 $Ha]") as "Hown". 
+              iApply ("IH" with "Hfull' Hreg' Hmap Hsts Hown"); auto. 
+            - destruct (H3 dst) as [wdst Hsomedst].
               assert (delete PC r !! dst = Some wdst) as Hsomedst'.
               { rewrite -Hsomedst. apply (lookup_delete_ne r PC dst). eauto. }
               assert (delete src (delete PC r) !! dst = Some wdst) as Hsomedst''.
@@ -610,17 +602,19 @@ Section fundamental.
               (* apply IH *)
               (* we will apply the IH on an updated register state *)
               (* we can only prove the following once we have taken a step *)
-              iAssert (interp_registers (<[src:=inr (p, l, a2, a1, a0)]> (<[dst:=w0]> r)))
-                        as "Hreg'".
-              { iIntros (r0). iDestruct ("Hreg" $! (r0)) as "[% Hv]".
-                destruct H2 as [c Hsome].
-                iSplit; auto.
-                - iPureIntro.
+              iAssert (▷ interp_registers _ _ (<[src:=inr (p, l, a2, a1, a0)]> (<[dst:=w0]> r)))%I
+                        as "[Hfull' Hreg']".
+              { iNext. iSplitR.
+                - iIntros (r0).
+                  destruct (H3 r0) as [c Hsome].
+                  iPureIntro.
                   destruct (decide (src = r0)); simplify_eq;
                     [rewrite lookup_insert|rewrite lookup_insert_ne]; eauto.
                   destruct (decide (dst = r0)); simplify_eq;
                     [rewrite lookup_insert|rewrite lookup_insert_ne]; eauto.
-                - iIntros (Hnepc) "/=".
+                - iIntros (r0) "%".
+                  destruct (H3 r0) as [c Hsome].
+                  iDestruct ("Hreg" $! (r0)) as "Hv".
                   destruct (decide (src = r0)); simplify_eq.
                   + rewrite /RegLocate lookup_insert. iApply "Hvsrc". 
                   + rewrite /RegLocate lookup_insert_ne; auto. 
@@ -629,63 +623,107 @@ Section fundamental.
                     * rewrite lookup_insert_ne. rewrite Hsome. iApply "Hv"; auto.
                       auto. 
               }
-              iApply ("IH" with "Hreg' Hmap Hsts").
-              iFrame "Hinv".
-              (* reestablish invariants *)
-              iApply "Hcls"; iFrame.
-              iDestruct (extract_from_region _ _ a with
-                "[Hal Hah Hregionl Hvalidl Hregionh Hvalidh Ha]") as "Hregion"; eauto.
-              iExists _,_,_; rewrite Ha'; iFrame. iExact "Hva". iFrame. 
-              iApply "Hcls'". iFrame. 
-          }              
-          (* Now the final step is to open the invariant for each possible condition *)
-          iDestruct "Hconds" as "[#Hro|#[Hrw|Hrwl]]".
+              iNext.
+              iMod ("Hcls'" with "[$Ha0 $Ha]") as "Hown". 
+              iApply ("IH" with "Hfull' Hreg' Hmap Hsts Hown"); auto. 
+          }
+          destruct (decide ((b,e) = (a2,a1))).
+          {
+            inversion e0; subst. 
+            (* no need to open any invariant *)
+            admit. 
+          }
+          iDestruct "Hconds" as "[[#Hro|#[Hrw|Hrwl]] %]".
           (* each condition is similar, but with some subtle differences for closing *)
           { iDestruct "Hro" as (ws0) "Hinv0".
             (* open the invariant to access a0 ↦ₐ _ *)
-            iInv (logN.@(a2, a1)) as "Hro_cond" "Hcls'";[admit|].
+            iMod (na_inv_open _ _ _ (logN.@(a2, a1)) with "Hinv0 Hown")
+              as "(Hro_cond & Hown & Hcls')"; auto.
+            { apply namespace_subseteq_difference; auto.
+              rewrite /namespace_subseteq_difference.
+              by apply ndot_ne_disjoint. 
+            }
+            rewrite /read_only_cond.
             iDestruct (extract_from_region _ _ a0 with "Hro_cond")
-            as (a0l w0 a0h)
-            "(Ha0l & Ha0h & Hregion0l & Hvalid0l & >Ha0 & #Hva0 & Hregion0h & Hvalid0h)";
+              as (a0l w0 a0h)
+                   "(Ha0l & Ha0h & Hregion0l & Hvalid0l & >Ha0 & #Hva0 & Hregion0h & Hvalid0h)";
               first (split; by apply Z.leb_le,Is_true_eq_true).
-            iApply "Hstep".
-            iExists w0. iFrame "Ha0 #". iIntros "Ha0".
-            iApply "Hcls'". iNext.
-            iApply (extract_from_region _ _ a0);
+            iApply "Hstep". iFrame "Hsts".
+            iExists w0. iFrame "Ha0 Hva0". 
+            iNext. iIntros "[Ha0 Ha]".
+            iDestruct (extract_from_region _ _ a0
+                         with "[Hregion0l Hvalid0l Hregion0h Hvalid0h Ha0 Ha0l Ha0h]")
+              as "Hregion";
               first (split; by apply Z.leb_le,Is_true_eq_true).
-            iFrame. iExists a0l, _, a0h. iFrame. iExact "Hva0".
+            { iFrame. iExists a0l, _, a0h. iFrame. iExact "Hva0". }
+            iMod ("Hcls'" with "[$Hown $Hregion]") as "Hown".
+            iDestruct (extract_from_region _ _ a
+                         with "[Hregionl Hvalidl Hregionh Hvalidh Ha Hal Hah]")
+              as "Hregion"; eauto. 
+            { iFrame. iExists al, _, ah. iFrame. iExact "Hva". }
+            iMod ("Hcls" with "[$Hown $Hregion]") as "Hown".
+            iModIntro. iFrame. 
           }
           { (* open the invariant to access a0 ↦ₐ _ *)
-            iInv (logN.@(a2, a1)) as "Hrw_cond" "Hcls'";[admit|].
-            iDestruct "Hrw_cond" as (ws0) "Hrw_cond". 
+            iMod (na_inv_open _ _ _ (logN.@(a2, a1)) with "Hrw Hown")
+              as "(Hrw_cond & Hown & Hcls')"; auto.
+            { apply namespace_subseteq_difference; auto.
+              rewrite /namespace_subseteq_difference.
+              by apply ndot_ne_disjoint. 
+            }
+            rewrite /read_only_cond.
+            iDestruct "Hrw_cond" as (ws0) "Hrw_cond".
             iDestruct (extract_from_region _ _ a0 with "Hrw_cond")
             as (a0l w0 a0h)
      "(Ha0l & Ha0h & Hregion0l & Hvalid0l & >Ha0 & #[Hva0 Hnl] & Hregion0h & Hvalid0h)";
               first (split; by apply Z.leb_le,Is_true_eq_true).
-            iApply "Hstep".
-            iExists w0. iFrame "Ha0 #". iIntros "Ha0".
-            iApply "Hcls'". iNext.
-            iDestruct (extract_from_region _ _ a0 with
-                "[Ha0l Ha0h Hregion0l Hvalid0l Hregion0h Hvalid0h Ha0]") as "Hregion0".
-            { split; apply Z.leb_le,Is_true_eq_true; eauto. }
-            { iExists a0l,_,a0h. iFrame. iFrame "#". }
-            iExists ws0. iFrame.
+            iApply "Hstep". iFrame. 
+            iExists w0. iFrame "Ha0 #".
+            iNext. iIntros "[Ha0 Ha]". 
+            iDestruct (extract_from_region _ _ a0
+                         with "[Hregion0l Hvalid0l Hregion0h Hvalid0h Ha0 Ha0l Ha0h]")
+              as "[Hbe Hregion]";
+              first (split; by apply Z.leb_le,Is_true_eq_true).
+            { iFrame. iExists a0l, _, a0h. iFrame. iFrame "#". } 
+            iMod ("Hcls'" with "[$Hown Hbe Hregion]") as "Hown".
+            { iNext. iExists _. iFrame. iApply big_sepL_later. iNext. iFrame. }
+            iDestruct (extract_from_region _ _ a
+                         with "[Hregionl Hvalidl Hregionh Hvalidh Ha Hal Hah]")
+              as "Hregion"; eauto. 
+            { iFrame. iExists al, _, ah. iFrame. iExact "Hva". }
+            iMod ("Hcls" with "[$Hown $Hregion]") as "Hown".
+            iModIntro. iFrame. 
           }
           { (* open the invariant to access a0 ↦ₐ _ *)
-            iInv (logN.@(a2, a1)) as "Hrw_cond" "Hcls'";[admit|].
-            iDestruct "Hrw_cond" as (ws0) "Hrw_cond". 
-            iDestruct (extract_from_region _ _ a0 with "Hrw_cond")
+            iMod (na_inv_open _ _ _ (logN.@(a2, a1)) with "Hrwl Hown")
+              as "(Hrwl_cond & Hown & Hcls')"; auto.
+            { apply namespace_subseteq_difference; auto.
+              rewrite /namespace_subseteq_difference.
+              by apply ndot_ne_disjoint. 
+            }
+            rewrite /read_only_cond.
+            iDestruct "Hrwl_cond" as (ws0) "Hrwl_cond".
+            iDestruct (extract_from_region _ _ a0 with "Hrwl_cond")
             as (a0l w0 a0h)
-            "(Ha0l & Ha0h & Hregion0l & Hvalid0l & >Ha0 & #Hva0 & Hregion0h & Hvalid0h)";
+     "(Ha0l & Ha0h & Hregion0l & Hvalid0l & >Ha0 & #Hva0 & Hregion0h & Hvalid0h)";
               first (split; by apply Z.leb_le,Is_true_eq_true).
-            iApply "Hstep".
-            iExists w0. iFrame "Ha0 #". iIntros "Ha0".
-            iApply "Hcls'". iNext.
-            iDestruct (extract_from_region _ _ a0 with
-                "[Ha0l Ha0h Hregion0l Hvalid0l Hregion0h Hvalid0h Ha0]") as "Hregion0".
-            { split; apply Z.leb_le,Is_true_eq_true; eauto. }
-            { iExists a0l,_,a0h. iFrame. iFrame "#". }
-            iExists ws0. iFrame. }
+            iApply "Hstep". iFrame. 
+            iExists w0. iFrame "Ha0 #".
+            iNext. iIntros "[Ha0 Ha]". 
+            iDestruct (extract_from_region _ _ a0
+                         with "[Hregion0l Hvalid0l Hregion0h Hvalid0h Ha0 Ha0l Ha0h]")
+              as "[Hbe Hregion]";
+              first (split; by apply Z.leb_le,Is_true_eq_true).
+            { iFrame. iExists a0l, _, a0h. iFrame. iFrame "#". } 
+            iMod ("Hcls'" with "[$Hown Hbe Hregion]") as "Hown".
+            { iNext. iExists _. iFrame. iApply big_sepL_later. iNext. iFrame. }
+            iDestruct (extract_from_region _ _ a
+                         with "[Hregionl Hvalidl Hregionh Hvalidh Ha Hal Hah]")
+              as "Hregion"; eauto. 
+            { iFrame. iExists al, _, ah. iFrame. iExact "Hva". }
+            iMod ("Hcls" with "[$Hown $Hregion]") as "Hown".
+            iModIntro. iFrame. 
+          }
       + admit. (* Store *)
       + admit. (* Lt *)
       + admit. (* Add *)
@@ -707,18 +745,22 @@ Section fundamental.
   { admit. }
   Admitted.
   
-  
-  Theorem fundamental (perm : Perm) b e g (a : Addr) :
-    (⌜perm = RX⌝ ∧ ∃ ws, (inv (logN .@ (b,e)) (read_only_cond b e ws interp)%I)) ∨
-    (⌜perm = RWX⌝ ∧ (inv (logN .@ (b,e)) (read_write_cond b e interp)%I)) ∨
-    (⌜perm = RWLX⌝ ∧ (inv (logN .@ (b,e)) (read_write_local_cond b e interp)%I)) -∗
-    ⟦ inr ((perm,g),b,e,a) ⟧ₑ.
+
+  Theorem fundamental (perm : Perm) b e g (a : Addr) stsf E r :
+    (⌜perm = RX⌝ ∧ ∃ ws, (na_inv logrel_nais (logN .@ (b,e))
+                                 (read_only_cond b e ws stsf E interp)%I)) ∨
+    (⌜perm = RWX⌝ ∧ (na_inv logrel_nais (logN .@ (b,e))
+                                 (read_write_cond b e stsf E interp)%I)) ∨
+    (⌜perm = RWLX⌝ ∧ (na_inv logrel_nais (logN .@ (b,e))
+                                 (read_write_local_cond b e stsf E interp)%I)) -∗
+    ⟦ inr ((perm,g),b,e,a) ⟧ₑ stsf E r.
   Proof. 
     iIntros "[#[-> Hinv] | [#[-> Hinv] | #[-> Hinv]]]".
     - iDestruct "Hinv" as (ws) "Hinv". by iApply fundamental_RX. 
-    - (* read and write condition, non local *) admit. 
-    - (* read and write condition, permit local *) admit. 
-Admitted. 
-          
+    - by iApply fundamental_RWX. 
+    - by iApply fundamental_RWLX.
+  Qed.  
+
+    
       
 End fundamental. 
